Kura/Walk.lean
@@ -2,618 +2,1883 @@ import Kura.Subgraph
 import Kura.Minor
 import Mathlib.Data.Finset.Lattice.Basic
 import Kura.Dep.List
-
+import Mathlib.Data.Nat.PartENat
 
 open Set Function List Nat
-variable {α β : Type*} {G H : Graph α β} {x y z : α} {e f g : β}
+variable {α β : Type*} {G H : Graph α β} {u v x y z : α} {e e' f g : β}
 namespace Graph
 
 
-inductive Walk (G : Graph α β) : α → α → Type (max u_1 u_2) where
-| nil ⦃u : α⦄ (h : u ∈ G.V) : G.Walk u u
-| cons ⦃u v w : α⦄ ⦃e : β⦄ (he : G.IsBetween e w u) (W : G.Walk u v) : G.Walk w v
+inductive Walk (α β : Type*) where
+| nil (u : α) : Walk α β
+| cons (u : α) (e : β) (W : Walk α β) : Walk α β
 
 namespace Walk
-variable {w w₁ : G.Walk x y} {w₂ : G.Walk y z}
+variable {w w₁ : Walk α β} {w₂ : Walk α β}
 
-def vx {x y : α} : G.Walk x y → List α
-| nil _hx => [x]
-| cons _hbtw W => x :: W.vx
+def Nonempty : Walk α β → Prop
+| nil _ => False
+| cons _ _ _ => True
+
+def start : Walk α β → α
+| nil x => x
+| cons x _ _ => x
+
+def finish : Walk α β → α
+| nil x => x
+| cons _ _ w => w.finish
+
+def ValidOn (w : Walk α β) (G : Graph α β) : Prop :=
+  match w with
+  | nil x => x ∈ G.V
+  | cons x e w => G.IsBetween e x w.start ∧ w.ValidOn G
+
+def vx : Walk α β → List α
+| nil x => [x]
+| cons x _e w => x :: w.vx
+
+instance : Membership α (Walk α β) where
+  mem w x := x ∈ w.vx
+
+instance [DecidableEq α] : Decidable (x ∈ w) := by
+  change Decidable (x ∈ w.vx)
+  infer_instance
 
 @[simp]
-lemma nil_vx (hx : x ∈ G.V) : (nil hx).vx = [x] := rfl
+lemma mem_iff : (x ∈ w) = (x ∈ w.vx) := rfl
 
-@[simp]
-lemma cons_vx (hbtw : G.IsBetween e x y) (W : G.Walk y z) :
-  (cons hbtw W).vx = x :: W.vx := rfl
-
-def edge {x y : α} : G.Walk x y → List β
+def edge : Walk α β → List β
 | nil _ => []
-| cons _hbtw W => by
-  rename_i e
-  exact e :: W.edge
+| cons _ e w => e :: w.edge
 
-@[simp]
-lemma nil_edge (hx : x ∈ G.V) : (nil hx).edge = [] := rfl
-
-@[simp]
-lemma cons_edge (hbtw : G.IsBetween e x y) (W : G.Walk y z) :
-  (cons hbtw W).edge = e :: W.edge := rfl
-
-def length {x y : α} : G.Walk x y → ℕ
+def length : Walk α β → ℕ
 | nil _ => 0
-| cons _hbtw W => W.length + 1
+| cons _ _ w => w.length + 1
+
+def concat : Walk α β → β → α → Walk α β
+| nil x, e, y => cons x e (nil y)
+| cons x e w, f, y => cons x e (w.concat f y)
+
+def dropLast : Walk α β → Walk α β
+| nil x => nil x
+| cons x _ (nil _) => nil x
+| cons x e (cons y e' w) => cons x e ((cons y e' w).dropLast)
+
+def append : Walk α β → Walk α β → Walk α β
+| nil _x, w => w
+| cons x e w, w' => cons x e (w.append w')
+
+def reverse : Walk α β → Walk α β
+| nil x => nil x
+| cons x e w => w.reverse.concat e x
+
+def startAt [DecidableEq α] (w : Walk α β) (u : α) (h : u ∈ w) : Walk α β :=
+  match w with
+  | nil x => nil x
+  | cons x e w =>
+    if hin : u ∈ w
+    then startAt w u hin
+    else cons x e w
 
 @[simp]
-lemma nil_length (hx : x ∈ G.V) : (nil hx).length = 0 := rfl
+lemma cons_length : (cons x e w).length = w.length + 1 := rfl
+
+lemma startAt_length_le [DecidableEq α] {w : Walk α β} (h : u ∈ w) : (startAt w u h).length ≤ w.length := by
+  match w with
+  | nil x => simp [startAt]
+  | cons x e w =>
+    simp only [startAt, cons_length]
+    split_ifs with hin
+    · have := startAt_length_le hin
+      omega
+    · simp
+
+def dedup [DecidableEq α] : Walk α β → Walk α β
+| nil x => nil x
+| cons x e w =>
+  if h : x ∈ w
+  then by
+    have := startAt_length_le h
+    exact (startAt w x h).dedup
+  else cons x e (dedup w)
+termination_by w => w.length
+
+@[simp] lemma cons_vx : (cons x e w).vx = x :: w.vx := rfl
+
+def endIf [DecidableEq α] {P : α → Prop} [DecidablePred P] (w : Walk α β) (h : ∃ u ∈ w.vx, P u) : Walk α β :=
+  match w with
+  | nil x => nil x
+  | cons x e w =>
+    if hP : P x
+    then nil x
+    else cons x e (endIf w (by simpa only [cons_vx, mem_cons, exists_eq_or_imp, hP, false_or] using h))
+
+@[simp] lemma nil_vx : (nil x : Walk α β).vx = [x] := rfl
+
+@[simp] lemma nil_edge : (nil x : Walk α β).edge = [] := rfl
+
+@[simp] lemma nil_length : (nil x : Walk α β).length = 0 := rfl
+
+@[simp] lemma nil_start : (nil x : Walk α β).start = x := rfl
+
+@[simp] lemma nil_finish : (nil x : Walk α β).finish = x := rfl
+
+@[simp] lemma nil_validOn_iff : (nil x : Walk α β).ValidOn G ↔ x ∈ G.V := by
+  simp only [ValidOn]
+
+@[simp] lemma nil_injective : Injective (nil : α → Walk α β) := by
+  rintro x y h
+  rwa [nil.injEq] at h
+
+@[simp] lemma cons_edge : (cons x e w).edge = e :: w.edge := rfl
+
+@[simp] lemma cons_start : (cons x e w).start = x := rfl
+
+@[simp] lemma cons_finish : (cons x e w).finish = w.finish := rfl
+
+@[simp] lemma cons_validOn (hw : w.ValidOn G) (he : G.IsBetween e x w.start) :
+  (cons x e w).ValidOn G := ⟨he, hw⟩
+
+@[simp] lemma cons_validOn_iff : (cons x e w).ValidOn G ↔ G.IsBetween e x w.start ∧ w.ValidOn G :=
+  ⟨fun h => h, fun h => h⟩
+
+lemma Nonempty.exists_cons : w.Nonempty → ∃ x e w', w = cons x e w' := by
+  induction w with
+  | nil x => simp only [Nonempty, reduceCtorEq, exists_false, imp_self]
+  | cons x e w ih => simp only [cons.injEq, exists_and_left, exists_eq', and_true, implies_true]
 
 @[simp]
-lemma cons_length (hbtw : G.IsBetween e x y) (W : G.Walk y z) :
-  (cons hbtw W).length = W.length + 1 := rfl
-
-def of_isBetween (h : G.IsBetween e x y) : G.Walk x y :=
-  cons h (nil h.vx_mem_right)
+lemma Nonempty.not_nil : ¬ (nil x : Walk α β).Nonempty := by
+  simp only [Nonempty, not_false_eq_true]
 
 @[simp]
-lemma of_isBetween_vx (h : G.IsBetween e x y) : (of_isBetween h).vx = [x, y] := rfl
+lemma Nonempty.cons_true : (cons x e w).Nonempty := by
+  simp only [Nonempty]
 
 @[simp]
-lemma of_isBetween_edge (h : G.IsBetween e x y) : (of_isBetween h).edge = [e] := rfl
+lemma Nonempty.not_iff : ¬ w.Nonempty ↔ ∃ x, w = nil x := by
+  match w with
+  | nil x => simp only [not_nil, not_false_eq_true, nil.injEq, exists_eq']
+  | cons x e w => simp only [Nonempty, not_true_eq_false, reduceCtorEq, exists_false]
+
+lemma vx_ne_nil : w.vx ≠ [] := by
+  match w with
+  | nil x => simp
+  | cons x e w => simp
 
 @[simp]
-lemma of_isBetween_length (h : G.IsBetween e x y) : (of_isBetween h).length = 1 := rfl
-
-lemma of_adj (h : G.Adj x y) : ∃ (W : G.Walk x y), W.length = 1 := by
-  obtain ⟨e, he⟩ := h
-  use of_isBetween he
-  exact rfl
-
-lemma of_reflAdj (h : G.reflAdj x y) : ∃ (W : G.Walk x y), W.length ≤ 1 := by
-  obtain hadj | ⟨rfl, hx⟩ := h
-  · obtain ⟨W, hW⟩ := of_adj hadj
-    use W
-    rw [hW]
-  · use nil hx
-    simp only [nil_length, _root_.zero_le]
-
-
-def append {x y z : α} (w₁ : G.Walk x y) (w₂ : G.Walk y z) : G.Walk x z :=
-  match w₁ with
-  | nil h => w₂
-  | cons hbtw W => cons hbtw (append W w₂)
+lemma mem_vx_nil_iff : x ∈ (nil u : Walk α β) ↔ x = u := by
+  simp only [mem_iff, nil_vx, mem_cons, not_mem_nil, or_false]
 
 @[simp]
-lemma append_vx :
-  (append w₁ w₂).vx = w₁.vx ++ List.tail w₂.vx := by
+lemma mem_vx_cons_iff : x ∈ (cons u e w) ↔ x = u ∨ x ∈ w := by
+  simp only [mem_iff, cons_vx, mem_cons]
+
+@[simp]
+lemma mem_edge_nil_iff : e ∈ (nil u : Walk α β).edge ↔ False := by
+  simp only [nil_edge, mem_nil_iff]
+
+@[simp]
+lemma mem_edge_cons_iff : e ∈ (cons u e' w).edge ↔ e = e' ∨ e ∈ w.edge := by
+  simp only [cons_edge, mem_cons]
+
+@[simp]
+lemma start_vx_mem : w.start ∈ w.vx := by
+  match w with
+  | nil x => simp only [nil_vx, nil_start, mem_cons, not_mem_nil, or_false]
+  | cons x e w => simp only [cons_vx, cons_start, mem_cons, true_or]
+
+lemma start_eq_vx_head {w : Walk α β} : w.start = w.vx.head vx_ne_nil := by
+  match w with
+  | nil x => rfl
+  | cons x e w => rfl
+
+@[simp]
+lemma finish_vx_mem {w : Walk α β} : w.finish ∈ w.vx := by
+  match w with
+  | nil x => simp
+  | cons x e w =>
+    simp only [cons_vx, cons_finish, mem_cons]
+    right
+    exact finish_vx_mem
+
+lemma finish_eq_vx_getLast {w : Walk α β} : w.finish = w.vx.getLast vx_ne_nil := by
+  match w with
+  | nil x => rfl
+  | cons x e w =>
+    simp only [cons_finish, cons_vx, ne_eq, vx_ne_nil, not_false_eq_true, getLast_cons]
+    apply finish_eq_vx_getLast
+
+lemma ValidOn.mem_of_mem_vx {w : Walk α β} (h : w.ValidOn G) (hmem : x ∈ w.vx) :
+    x ∈ G.V := by
+  match w with
+  | nil y =>
+    simp only [nil_vx, mem_cons, not_mem_nil, or_false] at hmem
+    subst x
+    exact h
+  | cons y e w =>
+    obtain ⟨hbtw, hVd⟩ := h
+    obtain rfl | h : x = y ∨ x ∈ w.vx := by simpa using hmem
+    · exact hbtw.vx_mem_left
+    · exact hVd.mem_of_mem_vx h
+
+lemma ValidOn.mem_of_mem_edge {w : Walk α β} (h : w.ValidOn G) (hmem : e ∈ w.edge) :
+    e ∈ G.E := by
+  match w with
+  | nil x => simp at hmem
+  | cons x e' w =>
+    obtain ⟨hbtw, hVd⟩ := h
+    obtain rfl | h : e = e' ∨ e ∈ w.edge := by simpa using hmem
+    · exact hbtw.edge_mem
+    · exact hVd.mem_of_mem_edge h
+
+/-- Properties of append operation -/
+@[simp]
+lemma append_vx : (append w₁ w₂).vx = w₁.vx.dropLast ++ w₂.vx := by
   induction w₁ with
-  | nil hx =>
-    match w₂ with
-    | nil hy => simp [append]
-    | cons hbtw W => simp [append]
-  | cons hbtw W ih => simp [append, ih]
+  | nil x => simp [append]
+  | cons x e w ih =>
+    simp only [append, cons_vx, ih]
+    rw [List.dropLast_cons_of_ne_nil vx_ne_nil]
+    simp
+
+lemma append_vx' (heq : w₁.finish = w₂.start) : (append w₁ w₂).vx = w₁.vx ++ w₂.vx.tail := by
+  induction w₁ with
+  | nil x =>
+    simp_all only [nil_finish, append_vx, nil_vx, dropLast_single, nil_append, cons_append]
+    rw [start_eq_vx_head]
+    exact (head_cons_tail w₂.vx vx_ne_nil).symm
+  | cons x e w ih =>
+    rw [append_vx] at ih
+    simp only [cons_finish, append_vx, cons_vx, cons_append] at heq ⊢
+    rw [List.dropLast_cons_of_ne_nil vx_ne_nil]
+    simp only [cons_append, List.cons.injEq, true_and]
+    exact ih heq
 
 @[simp]
-lemma append_edge :
-  (append w₁ w₂).edge = w₁.edge ++ w₂.edge := by
+lemma append_edge {w₁ w₂ : Walk α β} : (append w₁ w₂).edge = w₁.edge ++ w₂.edge := by
   induction w₁ with
-  | nil hx => simp [append]
-  | cons hbtw W ih => simp [append, ih]
-
-@[simp]
-lemma append_length :
-  (append w₁ w₂).length = w₁.length + w₂.length := by
-  induction w₁ with
-  | nil hx => simp [append]
-  | cons hbtw W ih =>
+  | nil x => simp [append]
+  | cons x e w ih =>
     simp [append, ih]
-    ring
 
-
-def concat {x y z : α} (w : G.Walk x y) {e : β} (h : G.IsBetween e y z) : G.Walk x z :=
-  append w (of_isBetween h)
-
-/-- The vertices of a concat walk combine the vertices of the original walk with the endpoint. -/
 @[simp]
-lemma concat_vx (h : G.IsBetween e y z) :
-  (concat w h).vx = w.vx ++ [z] := by
-  simp [concat]
+lemma append_length : (append w₁ w₂).length = w₁.length + w₂.length := by
+  induction w₁ with
+  | nil x => simp [append]
+  | cons x e w ih =>
+    simp only [append, cons_length, ih]
+    omega
 
-/-- The edges of a concat walk combine the edges of the original walk with the new edge. -/
 @[simp]
-lemma concat_edge (h : G.IsBetween e y z) : (concat w h).edge = w.edge ++ [e] := by
-  simp [concat]
-
-/-- The length of a concat walk is the length of the original walk plus one. -/
-@[simp]
-lemma concat_length (h : G.IsBetween e y z) : (concat w h).length = w.length + 1 := by
-  simp [concat]
-
-
-def reverse {x y : α} (w : G.Walk x y) : G.Walk y x :=
-  match w with
-  | nil h => nil h
-  | cons hbtw W => append (reverse W) (of_isBetween hbtw.symm)
-
-/-- The vertices of a reversed walk are the reversal of the original walk's vertices. -/
-@[simp]
-lemma reverse_vx : (reverse w).vx = w.vx.reverse := by
+lemma nil_append : (nil x).append w = w := by
   induction w with
-  | nil h => simp [reverse]
-  | cons hbtw W ih => simp [reverse, ih]
+  | nil y => simp [append]
+  | cons y e w ih => simp [append, ih]
 
-/-- The edges of a reversed walk are the reversal of the original walk's edges. -/
 @[simp]
-lemma reverse_edge : (reverse w).edge = w.edge.reverse := by
-  induction w with
-  | nil h => simp [reverse]
-  | cons hbtw W ih => simp [reverse, ih]
+lemma cons_append :
+  (cons x e w₁).append w₂ = cons x e (w₁.append w₂) := rfl
 
-/-- The length of a reversed walk equals the length of the original walk. -/
 @[simp]
-lemma reverse_length : (reverse w).length = w.length := by
+lemma append_nil (h : w.finish = x) : w.append (nil x) = w := by
   induction w with
-  | nil h => simp [reverse]
-  | cons hbtw W ih => simp [reverse, ih]
+  | nil u => aesop
+  | cons u e W ih =>
+    rw [cons_finish] at h
+    rw [cons_append, ih h]
 
-/-- Given a walk, and a vertex that is in the walk, we can construct a walk from that vertex
-to the end of the walk.
-In the presence of multiple occurrences of the vertex in the walk, this function will return the
-shortest possible walk. (i.e. start from the last occurrence of the vertex)
--/
-def startAt [DecidableEq α] {x y z : α} (w : G.Walk x y) (hz : z ∈ w.vx) : G.Walk z y := by
-  match w with
-  | nil hx =>
-    simp only [nil_vx, mem_cons, not_mem_nil, or_false] at hz
-    subst hz
-    exact nil hx
-  | cons hbtw W =>
-    if hin : z ∈ W.vx then
-      exact startAt W hin
-    else
-      simp only [cons_vx, mem_cons, hin, or_false] at hz
-      subst z
-      exact cons hbtw W
+@[simp]
+lemma append_start_of_eq (h : w₁.finish = w₂.start):
+  (w₁.append w₂).start = w₁.start := by
+  induction w₁ with
+  | nil x => simp [append, ← h]
+  | cons x e w ih => simp [append, ih]
 
--- lemma startAt_vx_rtakeWhlie [DecidableEq α] {x y z : α} (w : G.Walk x y) (hz : z ∈ w.vx) :
---   (w.startAt hz).vx = z :: w.vx.rtakeWhile (· ≠ z) := by
---   induction w with
---   | nil =>
---     simp only [nil_vx, mem_cons, not_mem_nil, or_false] at hz
---     subst hz
---     simp [startAt]
---   | cons hbtw W ih =>
---     unfold startAt
---     split_ifs with hin
---     · rw [ih hin, cons_vx, eq_comm]
---       congr 1
---       apply List.rtakeWhlie_cons_of_mem_neg (hain := hin)
---       simp
---     · simp only [ne_eq, decide_not, cons_vx]
---       expose_names
---       suffices (cons hbtw W).vx = z :: rtakeWhile (fun x ↦ !decide (x = z)) (w :: W.vx) by
---         convert this using 1
+@[simp]
+lemma append_start_of_nonempty (h : w₁.Nonempty) :
+  (w₁.append w₂).start = w₁.start := by
+  induction w₁ with
+  | nil x => simp only [Nonempty.not_nil] at h
+  | cons x e w ih => simp only [cons_append, cons_start]
 
---         sorry
---       sorry
+@[simp]
+lemma append_finish :
+  (w₁.append w₂).finish = w₂.finish := by
+  induction w₁ with
+  | nil x => simp only [append]
+  | cons x e w ih => simp only [append, cons_finish, ih]
 
+lemma append_validOn (h : w₁.finish = w₂.start) (h₁ : w₁.ValidOn G) (h₂ : w₂.ValidOn G) :
+  (append w₁ w₂).ValidOn G := by
+  induction w₁ with
+  | nil x => simpa
+  | cons x e w₁ ih =>
+    simp only [cons_finish] at h
+    refine ⟨?_, by simp [ih h h₁.2]⟩
+    convert h₁.1 using 1
+    exact append_start_of_eq h
 
+lemma ValidOn.append_left_validOn (h : w₁.finish = w₂.start) (hw₁ : w₁.Nonempty)
+    (hVd : (append w₁ w₂).ValidOn G) : w₁.ValidOn G := by
+  induction w₁ with
+  | nil x => simp only [Nonempty.not_nil] at hw₁
+  | cons x e w ih =>
+    simp only [cons_append, cons_validOn_iff] at hVd
+    by_cases hNonempty : w.Nonempty
+    · refine ⟨?_, ih h hNonempty hVd.2⟩
+      convert hVd.1 using 1
+      simp only [hNonempty, append_start_of_nonempty]
+    · simp only [Nonempty.not_iff] at hNonempty
+      obtain ⟨y, rfl⟩ := hNonempty
+      simp only [cons_finish, nil_finish, nil_append, cons_validOn_iff, nil_start,
+        nil_validOn_iff] at h hVd ⊢
+      subst y
+      refine ⟨hVd.1, hVd.2.mem_of_mem_vx start_vx_mem⟩
 
+lemma ValidOn.append_right_validOn (hVd : (append w₁ w₂).ValidOn G) : w₂.ValidOn G := by
+  induction w₁ with
+  | nil x => simpa only [nil_append] using hVd
+  | cons x e w ih =>
+    simp only [cons_append, cons_validOn_iff] at hVd
+    exact ih hVd.2
 
-/-- Given a walk, and a vertex that is in the walk, we can construct a walk from the start of the
-walk to that vertex.
-In the presence of multiple occurrences of the vertex in the walk, this function will return the
-shortest possible walk. (i.e. stop at the first occurrence of the vertex)
--/
-def endAt [DecidableEq α] {x y z : α} (w : G.Walk x y) (hz : z ∈ w.vx) : G.Walk x z :=
-  (w.reverse.startAt (by simpa)).reverse
+lemma ValidOn.finish_eq_start (hw₁ : w₁.Nonempty) (hVd₁ : w₁.ValidOn G) (hVd : (append w₁ w₂).ValidOn G) :
+  w₁.finish = w₂.start := by
+  induction w₁ with
+  | nil x => simp only [Nonempty.not_nil] at hw₁
+  | cons x e w ih =>
+    simp_all only [Nonempty.cons_true, cons_append, cons_validOn_iff, cons_finish, forall_const]
+    by_cases hNonempty : w.Nonempty
+    · simp_all only [forall_const, append_start_of_eq, true_and]
+    · simp only [Nonempty.not_iff] at hNonempty
+      obtain ⟨y, rfl⟩ := hNonempty
+      simp_all only [Nonempty.not_nil, nil_finish, IsEmpty.forall_iff, nil_start, nil_validOn_iff,
+        nil_append]
+      exact hVd₁.1.eq_of_IsBetween hVd.1
 
--- def dedup [DecidableEq α] {x y : α} (w : G.Walk x y) : G.Walk x y :=
---   match w with
---   | nil hx => nil hx
---   | cons hbtw W =>
---     if hin : x ∈ W.vx
---     then (W.startAt hin).dedup
---     else cons hbtw (dedup W)
+end Walk
 
--- lemma dedup_vx_nodup [DecidableEq α] (w : G.Walk x y) : w.dedup.vx.Nodup := by
---   match w with
---   | nil hx => simp [dedup]
---   | cons hbtw W =>
---     simp only [dedup]
---     split_ifs with hin
---     · simp [startAt]
---     · simp
+open Walk
 
+variable {G H : Graph α β} {u v : α} {e : β} {w : Walk α β}
 
+def IsBetween.walk (_h : G.IsBetween e u v) : Walk α β := cons u e (nil v)
 
-lemma connected (W : G.Walk x y) : G.Connected x y := by
-  induction W with
-  | nil h => exact Connected.refl h
-  | cons W hbtw ih =>
-    rename_i u v w e
-    refine Connected.trans ?_ ih
-    refine Adj.connected ?_
-    use e
+lemma IsBetween.walk_validOn (h : G.IsBetween e u v) : h.walk.ValidOn G := by
+  simp only [walk, ValidOn, h.vx_mem_right, nil_start, h, cons_validOn]
 
-lemma connected_iff : G.Connected x y ↔ Nonempty (G.Walk x y) := by
-  refine ⟨fun h ↦ ?_, fun a ↦ a.some.connected⟩
+@[simp] lemma IsBetween.Walk.start (h : G.IsBetween e u v): h.walk.start = u := rfl
+
+@[simp] lemma IsBetween.Walk.finish (h : G.IsBetween e u v): h.walk.finish = v := rfl
+
+@[simp] lemma IsBetween.Walk.vx (h : G.IsBetween e u v): h.walk.vx = [u, v] := rfl
+
+@[simp] lemma IsBetween.Walk.edge (h : G.IsBetween e u v): h.walk.edge = [e] := rfl
+
+@[simp] lemma IsBetween.Walk.length (h : G.IsBetween e u v): h.walk.length = 1 := rfl
+
+lemma IsBetween.mem_left_of_edge_mem_walk (h : G.IsBetween e u v) (he : e ∈ w.edge)
+    (hVd : w.ValidOn G) : u ∈ w.vx := by
+  induction w with
+  | nil x => simp at he
+  | cons x e' w ih =>
+    simp only [cons_edge, mem_cons, cons_vx] at he ⊢
+    obtain rfl | he' := he
+    · obtain ⟨hbtw, hVd⟩ := hVd
+      obtain ⟨rfl, rfl⟩ | ⟨rfl, rfl⟩ := hbtw.eq_or_eq_of_IsBetween h
+      · left
+        rfl
+      · right
+        exact start_vx_mem
+    · right
+      exact ih he' hVd.2
+
+lemma IsBetween.mem_right_of_edge_mem_walk (h : G.IsBetween e u v) (he : e ∈ w.edge)
+    (hVd : w.ValidOn G) : v ∈ w.vx := h.symm.mem_left_of_edge_mem_walk he hVd
+
+/-- Given a graph adjacency, we can create a walk of length 1 -/
+lemma Adj.exist_walk (h : G.Adj u v) : ∃ (W : Walk α β), W.ValidOn G ∧ W.length = 1 ∧ W.start = u ∧
+    W.finish = v := by
+  obtain ⟨e, he⟩ := h
+  use he.walk, he.walk_validOn
+  simp only [IsBetween.Walk.length, IsBetween.Walk.start, IsBetween.Walk.finish, and_self]
+
+/-- Given a reflexive adjacency, we can create a walk of length at most 1 -/
+lemma reflAdj.exist_walk (h : G.reflAdj u v) : ∃ (W : Walk α β), W.ValidOn G ∧ W.length ≤ 1 ∧
+    W.start = u ∧ W.finish = v := by
+  obtain hadj | ⟨rfl, hx⟩ := h
+  · obtain ⟨W, hW, hlength, hstart, hfinish⟩ := hadj.exist_walk
+    use W, hW
+    simp only [hlength, le_refl, hstart, hfinish, and_self]
+  · use nil u
+    constructor
+    · simp [ValidOn, hx]
+    · simp
+
+lemma Connected.exist_walk (h : G.Connected u v) : ∃ (W : Walk α β), W.ValidOn G ∧
+    W.start = u ∧ W.finish = v := by
   induction h with
   | single hradj =>
-    obtain ⟨W, hW⟩ := of_reflAdj hradj
+    obtain ⟨W, hW, hlength, hstart, hfinish⟩ := hradj.exist_walk
     use W
-  | tail hConn hrAdj ih =>
-    obtain ⟨W', hW'⟩ := of_reflAdj hrAdj
-    use ih.some.append W'
+  | tail hconn hradj ih =>
+    expose_names
+    obtain ⟨W, hW, hstart, hfinish⟩ := ih
+    obtain ⟨W', hW', hlength, hstart', hfinish'⟩ := hradj.exist_walk
+    subst b c u
+    use W.append W', append_validOn hstart'.symm hW hW'
+    simp only [hstart', append_start_of_eq, append_finish, and_self]
 
-def le {x y : α} {H : Graph α β} (w : G.Walk x y) (hle : G ≤ H) : H.Walk x y :=
+lemma Walk.connected_of_validOn (h : w.ValidOn G) : G.Connected w.start w.finish := by
+  induction w with
+  | nil x => simpa only [nil_start, nil_finish, Connected.refl_iff]
+  | cons x e w ih =>
+    obtain ⟨H1, H2⟩ := h
+    simp only [cons_start, cons_finish]
+    exact H1.connected.trans (ih H2)
+
+lemma Walk.connected_of_validOn_of_mem' (h : w.ValidOn G) (hx : u ∈ w.vx) :
+    G.Connected u w.finish := by
+  induction w generalizing u with
+  | nil x =>
+    simp only [nil_vx, mem_cons, not_mem_nil, or_false] at hx
+    subst u
+    simp only [nil_finish, Connected.refl_iff]
+    exact h
+  | cons x e w ih =>
+    simp only [cons_vx, mem_cons] at hx
+    obtain rfl | hx := hx
+    · exact Connected.trans h.1.connected (ih h.2 (start_vx_mem))
+    · exact ih h.2 hx
+
+lemma Walk.connected_of_validOn_of_mem (h : w.ValidOn G) (hx : x ∈ w.vx) (hy : y ∈ w.vx) :
+    G.Connected x y := by
+  have hx' := Walk.connected_of_validOn_of_mem' h hx
+  have hy' := Walk.connected_of_validOn_of_mem' h hy
+  exact Connected.trans hx' hy'.symm
+
+theorem Connected.iff_walk : G.Connected u v ↔ ∃ w : Walk α β, w.ValidOn G ∧ w.start = u ∧ w.finish = v := by
+  constructor
+  · exact fun a ↦ exist_walk a
+  · rintro ⟨w, h1, rfl, rfl⟩
+    exact connected_of_validOn h1
+
+
+namespace Walk
+
+/-- Properties of dropLast operation -/
+@[simp]
+lemma dropLast_vx {w : Walk α β} (h : w.Nonempty) : (w.dropLast).vx = w.vx.dropLast := by
   match w with
-  | nil h => nil (vx_subset_of_le hle h)
-  | cons hbtw W => cons (hbtw.le hle) (W.le hle)
+  | .nil x => simp only [Nonempty.not_nil] at h
+  | .cons x e (.nil y) => simp only [dropLast, nil_vx, cons_vx, dropLast_cons₂, dropLast_single]
+  | .cons x e (cons y e' w) =>
+    simp only [dropLast, cons_vx, dropLast_cons₂, List.cons.injEq, true_and]
+    rw [← cons_vx (e := e')]
+    apply dropLast_vx (by simp)
 
 @[simp]
-lemma le_vx {x y : α} {w : G.Walk x y} (hle : G ≤ H) : (le w hle).vx = w.vx := by
+lemma dropLast_start {w : Walk α β} (h : w.Nonempty) : (w.dropLast).start = w.start := by
   match w with
-  | nil h => simp [le, nil_vx]
-  | cons hbtw W =>
-    simp only [le, cons_vx, List.cons.injEq, true_and]
-    exact W.le_vx hle
+  | .nil x => simp only [Nonempty.not_nil] at h
+  | .cons x e (.nil y) => simp only [dropLast, nil_start, cons_start]
+  | .cons x e (cons y e' w) => simp only [dropLast, cons_start]
+
+lemma dropLast_validOn {w : Walk α β} (hVd : w.ValidOn G) :
+    (w.dropLast).ValidOn G := by
+  match w with
+  | .nil x => simp only [dropLast, hVd]
+  | .cons x e (.nil y) =>
+    simp only [cons_validOn_iff, nil_start, nil_validOn_iff] at hVd
+    exact hVd.1.vx_mem_left
+  | .cons x e (cons y e' w) =>
+    rw [dropLast, cons_validOn_iff, dropLast_start (by simp)]
+    rw [cons_validOn_iff] at hVd
+    refine ⟨hVd.1, ?_⟩
+    exact dropLast_validOn hVd.2
+
+/-- Properties of concat operation -/
+@[simp]
+lemma concat_vx {w : Walk α β} {e : β} {v : α} : (w.concat e v).vx = w.vx ++ [v] := by
+  induction w with
+  | nil x => simp [concat]
+  | cons x e w ih => simp [concat, ih]
 
 @[simp]
-lemma le_edge {x y : α} {w : G.Walk x y} (hle : G ≤ H) : (le w hle).edge = w.edge := by
-  match w with
-  | nil h => simp [le]
-  | cons hbtw W =>
-    simp only [le, cons_edge, List.cons.injEq, true_and]
-    exact W.le_edge hle
+lemma concat_edge {w : Walk α β} {e : β} {v : α} : (w.concat e v).edge = w.edge ++ [e] := by
+  induction w with
+  | nil x => simp [concat]
+  | cons x e w ih => simp [concat, ih]
 
 @[simp]
-lemma le_length {x y : α} {w : G.Walk x y} (hle : G ≤ H) : (le w hle).length = w.length := by
-  match w with
-  | nil h => simp [le]
-  | cons hbtw W =>
-    simp only [le, cons_length, true_and]
-    have := W.le_length hle
-    exact congrFun (congrArg _ this) 1
+lemma concat_length {w : Walk α β} {e : β} {v : α} : (w.concat e v).length = w.length + 1 := by
+  induction w with
+  | nil x => simp [concat]
+  | cons x e w ih => simp [concat, ih]
 
--- def contract {α' : Type*} {x' y' : α'} {f : α → α'} {C : Set β} (w : (G /[f] C).Walk x' y')
---     (hx : f x = x') (hy : f y = y') : G.Walk x y := by
+/-- Properties of reverse operation -/
+@[simp]
+lemma reverse_vx {w : Walk α β} : (reverse w).vx = w.vx.reverse := by
+  induction w with
+  | nil x => simp [reverse]
+  | cons x e w ih => simp [reverse, ih]
+
+@[simp]
+lemma reverse_edge {w : Walk α β} : (reverse w).edge = w.edge.reverse := by
+  induction w with
+  | nil x => simp [reverse]
+  | cons x e w ih => simp [reverse, ih]
+
+@[simp]
+lemma reverse_length {w : Walk α β} : (reverse w).length = w.length := by
+  induction w with
+  | nil x => simp [reverse]
+  | cons x e w ih => simp [reverse, ih]
+
+
+
+lemma eq_append_cons_of_edge_mem {w : Walk α β} {e : β} (he : e ∈ w.edge) :
+    ∃ w₁ w₂ : Walk α β, w = w₁.append (cons w₁.finish e w₂) ∧ e ∉ w₁.edge := by
+  induction w with
+  | nil x => simp only [nil_edge, not_mem_nil] at he
+  | cons x e' w ih =>
+    simp only [cons_edge, mem_cons] at he
+    obtain rfl | he' := he
+    · use nil x, w, rfl, by simp only [nil_edge, not_mem_nil, not_false_eq_true]
+    · by_cases h : e = e'
+      · subst e'
+        use nil x, w, rfl, by simp only [nil_edge, not_mem_nil, not_false_eq_true]
+      · obtain ⟨w₁, w₂, rfl, hnin⟩ := ih he'
+        use cons x e' w₁, w₂, by simp only [cons_finish, cons_append]
+        simp only [cons_edge, mem_cons, h, hnin, or_self, not_false_eq_true]
+
+/-- A subgraph inherits all valid walks -/
+lemma ValidOn.le {w : Walk α β} (h : w.ValidOn G) (hle : G ≤ H) : w.ValidOn H := by
+  match w with
+  | nil x => exact vx_subset_of_le hle h
+  | cons x e w =>
+    obtain ⟨hbtw, hVd⟩ := h
+    exact ⟨hbtw.le hle, hVd.le hle⟩
+
+lemma ValidOn.eq_nil_of_mem_isolated {w : Walk α β} {x : α} (hisol : G.Isolated x) (hmem : x ∈ w.vx)
+    (h : w.ValidOn G) : w = nil x := by
+  match w with
+  | nil y => simp_all only [nil_vx, mem_cons, not_mem_nil, or_false]
+  | cons y e w =>
+    exfalso
+    obtain ⟨hbtw, hVd⟩ := h
+    simp only [cons_vx, mem_cons] at hmem
+    obtain rfl | h := hmem
+    · exact hisol e hbtw.inc_left
+    · have := ValidOn.eq_nil_of_mem_isolated hisol h hVd
+      subst w
+      rw [nil_start] at hbtw
+      exact hisol e hbtw.inc_right
+
+lemma ValidOn.induce {U : Set α} (hVd : w.ValidOn G) (hU : ∀ x ∈ w.vx, x ∈ U) :
+    w.ValidOn (G[U]) := by
+  induction w with
+  | nil x => simp only [ValidOn, induce_V, nil_vx, mem_cons, not_mem_nil, or_false, hU]
+  | cons x e w ih =>
+    obtain ⟨hbtw, hVd⟩ := hVd
+    simp only [cons_vx, mem_cons, forall_eq_or_imp] at hU
+    obtain ⟨hUx, hUw⟩ := hU
+    refine ⟨?_, ih hVd hUw⟩
+    simp only [induce_isBetween_iff, hbtw, true_and, hUx]
+    exact hUw _ start_vx_mem
+
+lemma ValidOn.restrict {S : Set β} (hVd : w.ValidOn G) (hS : ∀ e ∈ w.edge, e ∈ S) :
+    w.ValidOn (G{S}) := by
+  induction w with
+  | nil x => exact hVd
+  | cons x e w ih =>
+    obtain ⟨hbtw, hVd⟩ := hVd
+    specialize ih hVd ?_
+    · rintro e' he'
+      refine hS e' ?_
+      simp only [cons_edge, mem_cons, he', or_true]
+    have he : e ∈ S := by
+      apply hS
+      simp only [cons_edge, mem_cons, true_or]
+    simp only [ih, restrict_isBetween, hbtw, he, and_self, cons_validOn]
+
+lemma ValidOn.subgraph {U : Set α} {S : Set β} (hVd : w.ValidOn G) (hU : ∀ x ∈ w.vx, x ∈ U)
+    (hS : ∀ e ∈ w.edge, e ∈ S) : w.ValidOn (G{S}[U]) := ValidOn.induce (ValidOn.restrict hVd hS) hU
+
+end Walk
+-- noncomputable def Contract.walk {α' : Type*} {w : Walk α' β} {p : α → α'} {C : Set β}
+--     (hVd : ValidOn G p C) (h : w.ValidOn (G /[p] C)) {x y : α} (hx : x ∈ G.V) (hy : y ∈ G.V)
+--     (hpx : p x = w.start) (hpy : p y = w.finish) : Walk α β :=
 --   match w with
---   | nil hx' =>
---     subst x'
+--   | .nil u => ((hVd hx hy).mp <| hpx.trans hpy.symm).symm.exist_walk.choose
+--   | .cons u e W => by
+--     have hw : (Walk.cons u e W).ValidOn ((G /[p] C){{e | e ∈ (Walk.cons u e W).edge}}) :=
+--       ValidOn.restrict _ _ h (by simp)
+--     simp only [cons_start, cons_finish] at hpx hpy
+--     simp only [cons_edge, mem_cons, cons_validOn_iff, restrict_isBetween, IsBetween, mem_setOf_eq,
+--       true_or, and_true] at hw
+--     simp only [cons_validOn_iff, IsBetween] at h
+--     obtain ⟨H, _hVdW⟩ := hw
+--     choose z hrfl a ha hbtw he using H
+--     subst hrfl
+--     rw [hVd hx hbtw.vx_mem_left] at hpx
+--     let w' := hpx.exist_walk.choose
+--     exact w'.append (Walk.cons w'.finish e <| walk hVd h.2 hbtw.vx_mem_right hy ha hpy)
 
---     subst hx'
---     exact nil hx
---   | cons hbtw W =>
---     simp only [cons_vx, cons_edge, cons_length]
+-- noncomputable def Contract.walk {α' : Type*} {w : Walk α' β} {p : α → α'} {C : Set β}
+--     (hVd : ValidOn G p C) (h : w.ValidOn (G /[p] C)) :
+--     ∀ x ∈ G.V, ∀ y ∈ G.V, p x = w.start → p y = w.finish → Walk α β := by
+--   induction w with
+--   | nil u =>
+--     rintro x hx y hy hpx hpy
+--     simp only [nil_start, nil_finish] at hpx hpy
+--     subst u
+--     rw [hVd hy hx] at hpy
+--     exact hpy.symm.exist_walk.choose
+--   | cons u e W ih =>
+--     rintro x hx y hy hpx hpy
+--     have hw : (Walk.cons u e W).ValidOn ((G /[p] C){{e | e ∈ (Walk.cons u e W).edge}}) := by
+--       apply ValidOn.restrict _ _ h ?_
+--       simp
+--     simp only [cons_start, cons_finish] at hpx hpy
+--     simp only [cons_edge, mem_cons, cons_validOn_iff, restrict_isBetween, IsBetween, mem_setOf_eq,
+--       true_or, and_true] at hw
+--     simp only [cons_validOn_iff, IsBetween] at h
+--     obtain ⟨H, _hVdW⟩ := hw
+--     choose z hrfl a ha hbtw he using H
+--     subst hrfl
+--     rw [hVd hx hbtw.vx_mem_left] at hpx
+--     let w' := hpx.exist_walk.choose
+--     exact w'.append (Walk.cons w'.finish e <| ih h.2 a hbtw.vx_mem_right y hy ha hpy)
 
+-- lemma Contract.walk_validOn {α' : Type*} {w : Walk α' β} {p : α → α'} {C : Set β}
+--     (hVd : ValidOn G p C) (h : w.ValidOn (G /[p] C)) (hx : x ∈ G.V) (hy : y ∈ G.V)
+--     (hpx : p x = w.start) (hpy : p y = w.finish) :
+--     (Contract.walk hVd h hx hy hpx hpy).ValidOn G := by
+--   match w with
+--   | .nil u =>
+--     unfold Contract.walk
+--     obtain ⟨H1, H2, H3⟩ := ((hVd hx hy).mp <| hpx.trans hpy.symm).symm.exist_walk.choose_spec
+--     exact H1.le (restrict_le _ _)
+--   | .cons u e W =>
+--     have hw : (Walk.cons u e W).ValidOn ((G /[p] C){{e | e ∈ (Walk.cons u e W).edge}}) :=
+--       ValidOn.restrict _ _ h (by simp)
+--     simp only [cons_start, cons_finish] at hpx hpy
+--     simp only [cons_edge, mem_cons, cons_validOn_iff, restrict_isBetween, IsBetween, mem_setOf_eq,
+--       true_or, and_true] at hw
+--     simp only [cons_validOn_iff, IsBetween] at h
+--     obtain ⟨H, _hVdW⟩ := hw
+--     choose z hrfl a ha hbtw he using H
+--     subst hrfl
+--     rw [hVd hx hbtw.vx_mem_left] at hpx
+--     let w' := hpx.exist_walk.choose
+--     unfold Contract.walk
+--     -- change (w'.append (Walk.cons w'.finish e <| walk hVd h.2 hbtw.vx_mem_right hy ha hpy)).ValidOn G
+--     sorry
+
+lemma Contract.walk {α' : Type*} {w : Walk α' β} {p : α → α'} {C : Set β} (hVd : ValidOn G p C)
+    (h : w.ValidOn (G /[p] C)) : ∀ x ∈ G.V, ∀ y ∈ G.V, p x = w.start → p y = w.finish →
+    ∃ w' : Walk α β, w'.ValidOn G ∧ w'.start = x ∧ w'.finish = y ∧
+    {e | e ∈ w'.edge} ⊆ {e | e ∈ w.edge ∨ e ∈ C} := by
+  induction w with
+  | nil u =>
+    rintro x hx y hy hpx hpy
+    simp only [nil_start, nil_finish] at hpx hpy
+    subst u
+    rw [hVd hy hx] at hpy
+    obtain ⟨w, hwVd, rfl, rfl⟩ := hpy.symm.exist_walk
+    use w, ?_, rfl, rfl
+    · simp only [nil_edge, not_mem_nil, false_or, setOf_mem_eq]
+      rintro e he
+      have := hwVd.mem_of_mem_edge he
+      exact Set.mem_of_mem_inter_right this
+    · exact hwVd.le (restrict_le _ _)
+  | cons u e W ih =>
+    rintro x hx y hy hpx hpy
+    have hw : (Walk.cons u e W).ValidOn ((G /[p] C){{e | e ∈ (Walk.cons u e W).edge}}) := by
+      apply ValidOn.restrict h ?_
+      simp
+    simp only [cons_start, cons_finish] at hpx hpy
+    simp only [cons_edge, mem_cons, cons_validOn_iff, restrict_isBetween, IsBetween, mem_setOf_eq,
+      true_or, and_true] at hw
+    simp only [cons_validOn_iff, IsBetween] at h
+    obtain ⟨⟨z, rfl, a, ha, hbtw, he⟩, hVdW⟩ := hw
+    obtain ⟨_B, hVdWp⟩ := h
+    rw [hVd hx hbtw.vx_mem_left] at hpx
+    obtain ⟨w, hVdw, rfl, rfl, hsu⟩ := ih hVdWp a hbtw.vx_mem_right y hy ha hpy
+    obtain ⟨w', hw'Vd, rfl, rfl⟩ := hpx.exist_walk
+    use w'.append (Walk.cons w'.finish e w), ?_, by simp, by simp
+    · simp +contextual only [append_edge, cons_edge, mem_append, mem_cons, setOf_subset_setOf]
+      rintro f (hfw' | rfl | hfw)
+      · right
+        have := hw'Vd.mem_of_mem_edge hfw'
+        exact Set.mem_of_mem_inter_right this
+      · tauto
+      · obtain (h1 | h2) := hsu hfw <;> tauto
+    · refine append_validOn (by simp) (hw'Vd.le (restrict_le _ _)) ?_
+      simp [hVdw, hbtw]
+
+lemma Contract.map_walk_of_walk {α' : Type*} {w : Walk α β} {p : α → α'} {C : Set β}
+    (hVd : ValidOn G p C) (h : w.ValidOn G) : ∃ w' : Walk α' β, w'.ValidOn (G /[p] C) ∧
+    w'.start = p w.start ∧ w'.finish = p w.finish ∧ {e | e ∈ w'.edge} ⊆ {e | e ∈ w.edge} := by
+  induction w with
+  | nil u =>
+    use nil (p u), ?_, rfl, rfl, by simp
+    use u, h
+  | cons u e W ih =>
+    obtain ⟨hbtw, hVdW⟩ := h
+    obtain ⟨w', hw'Vd, hst, hfin, hsub⟩ := ih hVdW
+    by_cases he : e ∈ C
+    · have : p u = w'.start := by
+        rw [hst, hVd hbtw.vx_mem_left hbtw.vx_mem_right]
+        apply IsBetween.connected
+        rw [restrict_isBetween]
+        exact ⟨hbtw, he⟩
+      use w', hw'Vd, this.symm, hfin
+      simp only [cons_edge, mem_cons, setOf_subset_setOf]
+      exact fun a a_1 ↦ Or.symm (Or.intro_left (a = e) (hsub a_1))
+    · use (Walk.cons (p u) e w'), ?_, by simp, by simp [hfin]
+      · simp only [cons_edge, mem_cons, setOf_subset_setOf, forall_eq_or_imp, true_or, true_and]
+        rintro f hfw'
+        right
+        exact hsub hfw'
+      · simp only [hw'Vd, cons_validOn_iff, IsBetween, and_true]
+        use u, rfl, W.start, hst.symm, hbtw
+
+namespace Walk
+variable [DecidableEq α]
+
+@[simp]
+lemma startAt_nil (hx : x ∈ (nil u : Walk α β).vx) : (nil u).startAt x hx = nil x := by
+  simp only [nil_vx, mem_cons, not_mem_nil, or_false] at hx
+  subst u
+  rfl
+
+@[simp]
+lemma startAt_start (hx : x ∈ w.vx) : (w.startAt x hx).start = x := by
+  induction w with
+  | nil u =>
+    simp only [nil_vx, mem_cons, not_mem_nil, or_false] at hx
+    exact hx.symm
+  | cons u e W ih =>
+    simp only [mem_iff, cons_vx, mem_cons] at hx
+    unfold startAt
+    by_cases h : x ∈ W.vx
+    · simp only [mem_iff, h, ↓reduceDIte]
+      exact ih h
+    · simp only [h, or_false, mem_iff, ↓reduceDIte, cons_start] at hx ⊢
+      exact hx.symm
+
+@[simp]
+lemma startAt_finish (hx : x ∈ w.vx): (w.startAt x hx).finish = w.finish := by
+  induction w with
+  | nil u => rfl
+  | cons u e W ih =>
+    simp only [mem_iff, cons_vx, mem_cons] at hx
+    unfold startAt
+    by_cases h : x ∈ W.vx
+    · simp only [mem_iff, h, ↓reduceDIte]
+      exact ih h
+    · simp only [h, or_false, mem_iff, ↓reduceDIte, cons_finish]
+
+@[simp]
+lemma startAt_length (hx : x ∈ w.vx) : (w.startAt x hx).length ≤ w.length := by
+  induction w with
+  | nil u => simp only [startAt_nil, nil_length, le_refl]
+  | cons u e W ih =>
+    simp only [cons_vx, mem_cons] at hx
+    unfold startAt
+    by_cases h : x ∈ W.vx
+    · simp only [mem_iff, h, ↓reduceDIte, cons_length]
+      have := ih h
+      omega
+    · simp only [mem_iff, h, ↓reduceDIte, cons_length, le_refl]
+
+@[simp]
+lemma startAt_sizeOf_le (hx : x ∈ w.vx) : sizeOf (w.startAt x hx) ≤ sizeOf w := by
+  induction w with
+  | nil u => simp only [startAt_nil, nil.sizeOf_spec, sizeOf_default, add_zero, le_refl]
+  | cons u e W ih =>
+    simp only [cons_vx, mem_cons] at hx
+    unfold startAt
+    by_cases h : x ∈ W.vx
+    · simp only [mem_iff, h, ↓reduceDIte, cons.sizeOf_spec, sizeOf_default, add_zero]
+      have := ih h
+      omega
+    · simp only [mem_iff, h, ↓reduceDIte, le_refl]
+
+lemma startAt_validOn (hx : x ∈ w.vx) (hVd : w.ValidOn G) : (w.startAt x hx).ValidOn G := by
+  induction w with
+  | nil u => simpa [startAt]
+  | cons u e W ih =>
+    simp only [cons_vx, mem_cons] at hx
+    unfold startAt
+    by_cases h : x ∈ W.vx
+    · simp only [mem_iff, h, ↓reduceDIte]
+      exact ih h hVd.2
+    · simpa only [mem_iff, h, ↓reduceDIte]
+
+lemma startAt_vx_count (hx : x ∈ w.vx) : (w.startAt x hx).vx.count x = 1 := by
+  induction w with
+  | nil u =>
+    simp only [nil_vx, mem_cons, not_mem_nil, or_false] at hx
+    subst u
+    unfold startAt
+    simp
+  | cons u e W ih =>
+    simp only [cons_vx, mem_cons] at hx
+    unfold startAt
+    by_cases h : x ∈ W.vx
+    · simp only [mem_iff, h, ↓reduceDIte]
+      exact ih h
+    · simp only [h, or_false, mem_iff, ↓reduceDIte, cons_vx] at hx ⊢
+      subst u
+      simp only [count_cons_self, add_eq_right]
+      exact count_eq_zero.mpr h
+
+lemma startAt_isSuffix (hx : x ∈ w.vx) :
+    ∃ w' : Walk α β, w'.append (w.startAt x hx) = w := by
+  induction w generalizing x with
+  | nil u =>
+    simp only [nil_vx, mem_cons, not_mem_nil, or_false] at hx
+    subst u
+    use nil x
+    rfl
+  | cons u e W ih =>
+    simp only [cons_vx, mem_cons] at hx
+    unfold startAt
+    by_cases h : x ∈ W.vx
+    · simp only [mem_iff, h, ↓reduceDIte]
+      obtain ⟨w', hw'⟩ := ih h
+      use cons u e w'
+      simp [hw']
+    · simp only [h, or_false, mem_iff, ↓reduceDIte] at hx ⊢
+      subst u
+      use nil x
+      rfl
+
+lemma startAt_vx_sublist {w : Walk α β} {x : α} (hx : x ∈ w.vx) :
+    (w.startAt x hx).vx ⊆ w.vx := by
+  induction w with
+  | nil u =>
+    simp only [nil_vx, mem_cons, not_mem_nil, or_false] at hx
+    subst u
+    simp only [startAt_nil, nil_vx, List.Subset.refl]
+  | cons u e W ih =>
+    simp only [cons_vx, mem_cons] at hx
+    unfold startAt
+    by_cases h : x ∈ W.vx
+    · simp only [mem_iff, h, ↓reduceDIte, cons_vx]
+      refine (ih h).trans ?_
+      simp only [List.Subset.refl, subset_cons_of_subset]
+    · simp only [mem_iff, h, ↓reduceDIte, cons_vx, List.Subset.refl]
+
+lemma startAt_edge_sublist {w : Walk α β} (hx : x ∈ w.vx) :
+    (w.startAt x hx).edge ⊆ w.edge := by
+  induction w with
+  | nil u =>
+    simp only [nil_vx, mem_cons, not_mem_nil, or_false] at hx
+    subst u
+    simp only [startAt_nil, nil_edge, List.Subset.refl]
+  | cons u e W ih =>
+    simp only [cons_vx, mem_cons] at hx
+    unfold startAt
+    by_cases h : x ∈ W.vx
+    · simp only [mem_iff, h, ↓reduceDIte, cons_edge]
+      refine (ih h).trans ?_
+      simp only [List.Subset.refl, subset_cons_of_subset]
+    · simp only [mem_iff, h, ↓reduceDIte, cons_edge, List.Subset.refl]
+
+lemma dedup_start (w : Walk α β) : w.dedup.start = w.start := by
+  match w with
+  | .nil u =>
+    unfold dedup
+    rfl
+  | .cons u e W =>
+    unfold dedup
+    split_ifs with h
+    · rw [cons_start, dedup_start (W.startAt u h), startAt_start]
+    · rfl
+
+lemma dedup_finish (w : Walk α β) : w.dedup.finish = w.finish := by
+  match w with
+  | .nil u =>
+    unfold dedup
+    rfl
+  | .cons u e W =>
+    unfold dedup
+    split_ifs with h
+    · rw [cons_finish, dedup_finish (W.startAt u h), startAt_finish]
+    · simp only [cons_finish]
+      exact dedup_finish W
+
+lemma dedup_length (w : Walk α β) : w.dedup.length ≤ w.length := by
+  match w with
+  | .nil u =>
+    unfold dedup
+    simp only [nil_length, le_refl]
+  | .cons u e W =>
+    unfold dedup
+    split_ifs with h
+    · simp only [cons_length, ge_iff_le]
+      have := dedup_length (W.startAt u h)
+      have := startAt_length_le h
+      omega
+    · simp only [cons_length, add_le_add_iff_right, ge_iff_le]
+      exact dedup_length W
+
+lemma dedup_sizeOf_le (w : Walk α β) : sizeOf w.dedup ≤ sizeOf w := by
+  match w with
+  | .nil u =>
+    unfold dedup
+    simp only [nil.sizeOf_spec, sizeOf_default, add_zero, le_refl]
+  | .cons u e W =>
+    unfold dedup
+    split_ifs with h
+    · simp only [cons.sizeOf_spec, sizeOf_default, add_zero]
+      have := dedup_sizeOf_le (W.startAt u h)
+      have := startAt_sizeOf_le h
+      omega
+    · simp only [cons.sizeOf_spec, sizeOf_default, add_zero, add_le_add_iff_left, ge_iff_le]
+      exact dedup_sizeOf_le W
+
+lemma dedup_validOn {w : Walk α β} (hVd : w.ValidOn G) : w.dedup.ValidOn G := by
+  match w with
+  | .nil u =>
+    unfold dedup
+    exact hVd
+  | .cons u e W =>
+    unfold dedup
+    split_ifs with h
+    · simp only [mem_iff, h, ↓reduceDIte]
+      exact dedup_validOn (startAt_validOn h hVd.2)
+    · simp only [dedup_validOn hVd.2, cons_validOn_iff, and_true]
+      convert hVd.1 using 1
+      exact dedup_start W
+
+lemma dedup_vx_sublist {w : Walk α β} {x : α} (hx : x ∈ w.dedup.vx) : x ∈ w.vx := by
+  match w with
+  | .nil u =>
+    unfold dedup at hx
+    exact hx
+  | .cons u e W =>
+    unfold dedup at hx
+    split_ifs at hx with h
+    · simp only at hx
+      exact mem_of_mem_tail <| startAt_vx_sublist h <| dedup_vx_sublist hx
+    · simp only [cons_vx, mem_cons] at hx ⊢
+      exact hx.imp (·) dedup_vx_sublist
+
+lemma dedup_edge_sublist (w : Walk α β) : w.dedup.edge ⊆ w.edge := by
+  match w with
+  | .nil u =>
+    unfold dedup
+    simp only [nil_edge, List.Subset.refl]
+  | .cons u e W =>
+    unfold dedup
+    split_ifs with h
+    · simp only [cons_edge]
+      refine (dedup_edge_sublist (W.startAt u h)).trans ?_
+      refine (startAt_edge_sublist h).trans ?_
+      simp only [List.Subset.refl, subset_cons_of_subset]
+    · simp only [cons_edge, cons_subset, mem_cons, true_or, true_and]
+      refine (dedup_edge_sublist W).trans ?_
+      simp only [List.Subset.refl, subset_cons_of_subset]
+
+lemma dedup_vx_nodup (w : Walk α β) : w.dedup.vx.Nodup := by
+  match w with
+  | .nil u =>
+    unfold dedup
+    simp only [nil_vx, nodup_cons, not_mem_nil, not_false_eq_true, nodup_nil, and_self]
+  | .cons u e W =>
+    unfold dedup
+    split_ifs with h
+    · simp only [mem_iff, h, ↓reduceDIte]
+      exact dedup_vx_nodup (W.startAt u h)
+    · simp only [cons_vx, nodup_cons, dedup_vx_nodup W, and_true]
+      contrapose! h
+      exact dedup_vx_sublist h
+
+lemma dedup_edge_nodup {w : Walk α β} (hVd : w.ValidOn G) : w.dedup.edge.Nodup := by
+  match w with
+  | .nil u =>
+    unfold dedup
+    simp only [nil_edge, nodup_nil]
+  | .cons u e W =>
+    unfold dedup
+    split_ifs with h
+    · simp only [mem_iff, h, ↓reduceDIte]
+      exact dedup_edge_nodup (startAt_validOn h hVd.2)
+    · simp only [cons_edge, nodup_cons, dedup_edge_nodup hVd.2, and_true]
+      obtain ⟨hne, hVd⟩ := hVd
+      rintro he
+      exact h <| hne.mem_left_of_edge_mem_walk (dedup_edge_sublist W he) hVd
+
+variable {P : α → Prop} [DecidablePred P]
+
+/- Properties of `endIf` -/
+
+@[simp]
+lemma endIf_nil {x : α} (h : ∃ u ∈ nil x, P u) : (nil x : Walk α β).endIf h = nil x := rfl
+
+@[simp]
+lemma endIf_cons {x : α} {e : β} {w : Walk α β} (h : ∃ u ∈ cons x e w, P u) :
+    (cons x e w).endIf h = if hP : P x
+    then nil x
+    else cons x e (endIf w (by simp [hP] at h; exact h)) := by
+  match w with
+  | .nil u => rfl
+  | .cons u e' w' => rfl
+
+lemma endIf_start {w : Walk α β} (h : ∃ u ∈ w.vx, P u) :
+    (w.endIf h).start = w.start := by
+  match w with
+  | .nil x => simp only [endIf, nil_start]
+  | .cons x e w =>
+    simp only [endIf, cons_start]
+    split_ifs <;> rfl
+
+lemma endIf_finish {w : Walk α β} (h : ∃ u ∈ w.vx, P u) :
+    P (w.endIf h).finish := by
+  match w with
+  | .nil x => simpa only [endIf_nil, nil_finish, nil_vx, mem_cons, not_mem_nil, or_false,
+    exists_eq_left] using h
+  | .cons x e w =>
+    rw [endIf]
+    split_ifs with hPx
+    · simpa only [nil_finish]
+    · simp only [cons_vx, mem_cons, exists_eq_or_imp, hPx, false_or, cons_finish] at h ⊢
+      exact endIf_finish h
+
+lemma endIf_length {w : Walk α β} (h : ∃ u ∈ w.vx, P u) :
+    (w.endIf h).length ≤  w.length := by
+  match w with
+  | .nil x => simp only [endIf, nil_length, le_refl]
+  | .cons x e w =>
+    simp only [endIf, cons_length, ge_iff_le]
+    split_ifs with h
+    · simp only [nil_length, le_add_iff_nonneg_left, _root_.zero_le]
+    · simp only [cons_length, add_le_add_iff_right]
+      apply endIf_length
+
+lemma endIf_sizeOf_le {w : Walk α β} (h : ∃ u ∈ w.vx, P u) :
+    sizeOf (w.endIf h) ≤ sizeOf w := by
+  match w with
+  | .nil x => simp only [endIf, nil.sizeOf_spec, sizeOf_default, add_zero, le_refl]
+  | .cons x e w =>
+    simp only [endIf, cons.sizeOf_spec, sizeOf_default, add_zero, ge_iff_le]
+    split_ifs with h
+    · simp only [nil.sizeOf_spec, sizeOf_default, add_zero, le_add_iff_nonneg_right,
+      _root_.zero_le]
+    · simp only [cons.sizeOf_spec, sizeOf_default, add_zero, add_le_add_iff_left]
+      apply endIf_sizeOf_le
+
+lemma endIf_validOn {w : Walk α β} (h : ∃ u ∈ w.vx, P u) (hVd : w.ValidOn G) :
+    (w.endIf h).ValidOn G := by
+  match w with
+  | .nil x => simpa only [endIf, nil_validOn_iff]
+  | .cons x e w =>
+    simp only [endIf]
+    split_ifs with hPx
+    · rw [nil_validOn_iff]
+      simp only [cons_validOn_iff] at hVd
+      exact hVd.1.vx_mem_left
+    · rw [cons_validOn_iff] at hVd ⊢
+      refine ⟨?_, endIf_validOn _ hVd.2⟩
+      convert hVd.1 using 1
+      simp only [cons_vx, mem_cons, exists_eq_or_imp, hPx, false_or] at h
+      exact endIf_start h
+
+lemma endIf_vx_sublist {w : Walk α β} (h : ∃ u ∈ w.vx, P u) :
+    (w.endIf h).vx ⊆ w.vx := by
+  match w with
+  | .nil x => simp only [endIf, nil_vx, List.Subset.refl]
+  | .cons x e w =>
+    simp only [endIf, cons_vx]
+    split_ifs with h
+    · simp only [nil_vx, cons_subset, mem_cons, true_or, nil_subset, subset_cons_of_subset,
+        and_self]
+    · simp only [cons_vx, cons_subset, mem_cons, true_or, true_and]
+      refine List.Subset.trans ?_ (List.subset_cons_self _ _)
+      apply endIf_vx_sublist
+
+lemma endIf_mem_vx {w : Walk α β} (h : ∃ u ∈ w.vx, P u) (hv : v ∈ (w.endIf h).vx):
+    ¬ P v ∨ v = (w.endIf h).finish := by
+  match w with
+  | .nil x =>
+    simp_all only [endIf_nil, mem_iff, nil_vx, mem_cons, not_mem_nil, or_false, nil_finish, or_true]
+  | .cons x e w =>
+    simp only [endIf_cons]
+    split_ifs with hPx
+    · simp only [endIf_cons, hPx, ↓reduceDIte, mem_iff, nil_vx, mem_cons, not_mem_nil,
+      or_false] at hv
+      subst v
+      right
+      rfl
+    · simp_all only [endIf_cons, dite_false, mem_iff, cons_vx, mem_cons, cons_finish]
+      obtain rfl | hvmem := hv
+      · exact Or.inl hPx
+      · simp only [cons_vx, mem_cons, exists_eq_or_imp, hPx, false_or] at h
+        exact endIf_mem_vx h hvmem
+
+lemma endIf_dropLast_mem_vx {w : Walk α β} (h : ∃ u ∈ w.vx, P u) (hNonempty : (w.endIf h).Nonempty)
+    (hu : u ∈ (w.endIf h).dropLast.vx) : ¬ P u := by
+  match w with
+  | .nil x => simp_all only [endIf_nil, Nonempty.not_nil]
+  | .cons x e (nil y) =>
+    simp_all only [endIf_cons, endIf_nil, dite_eq_ite, dropLast_vx]
+    split_ifs at hu with hPx
+    · simp_all only [cons_vx, nil_vx, mem_cons, not_mem_nil, or_false, exists_eq_or_imp,
+      exists_eq_left, true_or, ite_true, Nonempty.not_nil]
+    · simp_all only [cons_vx, nil_vx, mem_cons, not_mem_nil, or_false, exists_eq_or_imp,
+      exists_eq_left, false_or, ite_false, Nonempty.cons_true, dropLast_cons₂, dropLast_single,
+      not_false_eq_true]
+  | .cons x e (cons y e' w) =>
+    by_cases hPx : P x
+    · simp_all
+    · by_cases hxu : u = x
+      · simp_all
+      · obtain ⟨v, hv, hv2⟩ := h
+        rw [cons_vx, mem_cons] at hv
+        obtain rfl | hvmem := hv
+        · simp_all
+        · have hexists : ∃ u ∈ (cons y e' w).vx, P u := by use v
+          by_cases hnonempty : ((cons y e' w).endIf hexists).Nonempty
+          · refine endIf_dropLast_mem_vx (w := cons y e' w) (by use v) hnonempty ?_
+            by_cases hPy : P y
+            · simp only [endIf_cons, hPy, ↓reduceDIte]
+              sorry
+            ·
+              -- simp only [endIf_cons, hPx, ↓reduceDIte] at hu
+              -- rw [dropLast_vx, cons_vx, List.dropLast_cons] at hu
+              -- simp_all
+              sorry
+          · simp only [Nonempty.not_iff] at hnonempty
+            obtain ⟨a, ha⟩ := hnonempty
+            simp_all
+
+
+lemma endIf_exists_isBetween_last {w : Walk α β} (h : ∃ u ∈ w.vx, P u) (hVd : w.ValidOn G)
+    (hNonempty : (w.endIf h).Nonempty) : ∃ v ∈ (w.endIf h).vx, ¬ P v ∧ ∃ e, G.IsBetween e v (w.endIf h).finish := by
+  match w with
+  | .nil x => simp_all only [endIf_nil, Nonempty.not_nil]
+  | .cons x e (nil y) =>
+    simp_all only [cons_validOn_iff, nil_start, nil_validOn_iff, endIf_cons, endIf_nil, dite_eq_ite]
+    split_ifs with hPx
+    · simp_all only [cons_vx, nil_vx, mem_cons, not_mem_nil, or_false, exists_eq_or_imp,
+      exists_eq_left, true_or, ite_true, Nonempty.not_nil]
+    · simp_all only [cons_vx, nil_vx, mem_cons, not_mem_nil, or_false, exists_eq_or_imp,
+      exists_eq_left, false_or, ite_false, Nonempty.cons_true, cons_finish, nil_finish,
+      not_false_eq_true, true_and, not_true_eq_false, false_and]
+      use e
+      exact hVd.1
+  | .cons x e (cons y e' w) =>
+    unfold endIf
+    split_ifs with hPx
+    · simp_all only [cons_validOn_iff, cons_start, endIf_cons, dite_true, Nonempty.not_nil]
+    · by_cases hPy : P y
+      · simp_all only [cons_validOn_iff, cons_start, endIf_cons, dite_true, dite_eq_ite, ite_false,
+        Nonempty.cons_true, cons_vx, nil_vx, mem_cons, not_mem_nil, or_false, cons_finish,
+        nil_finish, exists_eq_or_imp, not_false_eq_true, true_and, exists_eq_left,
+        not_true_eq_false, false_and]
+        use e
+        exact hVd.1
+      · let w' := cons y e' w
+        rw [cons_finish, cons_vx]
+        have h' : ∃ u ∈ w'.vx, P u := by
+          change ∃ u ∈ (cons x e w').vx, P u at h
+          simpa only [cons_vx, mem_cons, exists_eq_or_imp, hPx, false_or] using h
+        have hNonempty' : (w'.endIf h').Nonempty := by
+          simp only [endIf_cons, hPy, ↓reduceDIte, Nonempty.cons_true, w']
+        obtain ⟨a, ha, hh⟩ := endIf_exists_isBetween_last (w := w') h' hVd.2 hNonempty'
+        refine ⟨a, ?_, hh⟩
+        rw [mem_cons]
+        right
+        exact ha
 
 end Walk
 
 
-abbrev Path (G : Graph α β) (x y : α) := {P : G.Walk x y // P.vx.Nodup}
+noncomputable def dist {G : Graph α β} {u v : α} (h : G.Connected u v) : ℕ := by
+  classical
+  exact Nat.find (by
+    obtain ⟨w, hwVd, rfl, rfl⟩ := h.exist_walk
+    use w.length, w, hwVd
+    : ∃ n, ∃ w : Walk α β, w.ValidOn G ∧ w.start = u ∧ w.finish = v ∧ w.length = n)
 
+
+
+/-- A path is a walk with no duplicate vertices -/
+def Path (α β : Type*) [DecidableEq α] := {w : Walk α β // w.vx.Nodup}
+
+variable [DecidableEq α] {p : Path α β}
 namespace Path
-variable {p p₁ : G.Path x y} {p₂ : G.Path y z}
 
 @[simp]
-def vx {x y : α} : G.Path x y → List α
-| ⟨W, _hW⟩ => W.vx
+def ofWalk (w : Walk α β) : Path α β := ⟨w.dedup, w.dedup_vx_nodup⟩
+
+/-- A path is valid on a graph if its underlying walk is valid -/
+@[simp]
+def ValidOn (p : Path α β) (G : Graph α β) : Prop := p.val.ValidOn G
 
 @[simp]
-def edge {x y : α} : G.Path x y → List β
-| ⟨W, _hW⟩ => W.edge
+def start (p : Path α β) : α := p.val.start
 
 @[simp]
-def length {x y : α} : G.Path x y → ℕ
-| ⟨W, _hW⟩ => W.length
+def finish (p : Path α β) : α := p.val.finish
 
-def nil (hx : x ∈ G.V) : G.Path x x := ⟨Walk.nil hx, by simp⟩
+/-- List of vertices in a path -/
+@[simp]
+def vx (p : Path α β) : List α := p.val.vx
+
+/-- List of edges in a path -/
+@[simp]
+def edge (p : Path α β) : List β := p.val.edge
+
+/-- Length of a path -/
+@[simp]
+def length (p : Path α β) : ℕ := p.val.length
+
+/-- Create a nil path -/
+@[simp]
+def nil (x : α) : Path α β := ⟨Walk.nil x, by simp⟩
+
+lemma nil_injective : Injective (nil : α → Path α β) := by
+  rintro x y h
+  rwa [nil, nil, ← Subtype.val_inj, nil.injEq] at h
 
 @[simp]
-lemma nil_val (hx : x ∈ G.V) : (nil hx).1 = Walk.nil hx := rfl
-
-@[simp]
-lemma nil_vx (hx : x ∈ G.V) : (nil hx).vx = [x] := rfl
-
-@[simp]
-lemma nil_edge (hx : x ∈ G.V) : (nil hx).edge = [] := rfl
-
-@[simp]
-lemma nil_length (hx : x ∈ G.V) : (nil hx).length = 0 := rfl
-
-/-- Create a path from a single edge between two vertices. -/
-def of_isBetween (h : G.IsBetween e x y) (hnotLoop : x ≠ y) : G.Path x y :=
-  ⟨Walk.of_isBetween h, by simpa⟩
-
-@[simp]
-lemma of_isBetween_val (h : G.IsBetween e x y) (hnotLoop : x ≠ y):
-  (of_isBetween h hnotLoop).1 = Walk.of_isBetween h := rfl
-
-@[simp]
-lemma of_isBetween_vx (h : G.IsBetween e x y) (hnotLoop : x ≠ y):
-  (of_isBetween h hnotLoop).vx = [x, y] := rfl
-
-@[simp]
-lemma of_isBetween_edge (h : G.IsBetween e x y) (hnotLoop : x ≠ y):
-  (of_isBetween h hnotLoop).edge = [e] := rfl
-
-@[simp]
-lemma of_isBetween_length (h : G.IsBetween e x y) (hnotLoop : x ≠ y):
-  (of_isBetween h hnotLoop).length = 1 := rfl
-
-/-- If two vertices are adjacent, there exists a path of length 1 between them. -/
-lemma of_adj (h : G.Adj x y) (hnotLoop : x ≠ y):
-    ∃ (P : G.Path x y), P.length = 1 ∧ P.vx = [x, y] := by
-  obtain ⟨e, he⟩ := h
-  use of_isBetween he hnotLoop, ?_
-  · simp
-  · apply of_isBetween_length
-
-/-- If two vertices are reflexively adjacent, there exists a path of length at most 1 between them. -/
-lemma of_reflAdj (h : G.reflAdj x y) : ∃ (P : G.Path x y), P.length ≤ 1 ∧ x ∈ P.vx ∧ y ∈ P.vx := by
-  by_cases hxy : x = y
-  · -- If x = y, use the nil path
-    subst hxy
-    refine ⟨nil h.mem_left, ?_⟩
-    constructor
-    · -- nil length is 0, which is ≤ 1
-      simp only [nil_length]
-      exact zero_le_one
-    · -- x and y are in the vertices list (both are x)
-      simp only [nil_vx, List.mem_singleton]
-      exact ⟨True.intro, True.intro⟩
-  · -- If x ≠ y, then they must be adjacent with an edge
-    rcases h with hadj | ⟨rfl, _⟩
-    · -- They're adjacent through an edge
-      obtain ⟨e, he⟩ := hadj
-      refine ⟨of_isBetween he hxy, ?_⟩
-      constructor
-      · -- Length is exactly 1
-        simp only [of_isBetween_length]
-        exact le_refl 1
-      · -- Both vertices are in the path
-        simp only [of_isBetween_vx, List.mem_cons, List.mem_singleton]
-        exact ⟨Or.inl True.intro, Or.inr (Or.inl True.intro)⟩
-    · -- This case is impossible since x ≠ y but rfl : x = y
-      contradiction
-
-def cons (h : G.IsBetween e x y) (p : G.Path y z) (hx : x ∉ p.vx) : G.Path x z :=
-  ⟨Walk.cons h (p.1), by simpa [p.2]⟩
-
-@[simp]
-lemma cons_val (h : G.IsBetween e x y) (p : G.Path y z) (hx : x ∉ p.vx) :
-  (cons h p hx).1 = Walk.cons h p.1 := rfl
-
-@[simp]
-lemma cons_vx (h : G.IsBetween e x y) (p : G.Path y z) (hx : x ∉ p.vx) :
-  (cons h p hx).vx = x :: p.vx := by
-  simp [cons]
-
-@[simp]
-lemma cons_edge (h : G.IsBetween e x y) (p : G.Path y z) (hx : x ∉ p.vx) :
-  (cons h p hx).edge = e :: p.edge := by
-  simp [cons]
-
-@[simp]
-lemma cons_length (h : G.IsBetween e x y) (p : G.Path y z) (hx : x ∉ p.vx) :
-  (cons h p hx).length = p.length + 1 := by
-  simp [cons]
-
-/-- Extend a path by an edge while maintaining the path property. -/
-def concat (p : G.Path x y) (h : G.IsBetween e y z) (hz : z ∉ p.vx) : G.Path x z :=
-  ⟨p.1.concat h, by
-    simp only [Walk.concat_vx]
-    rw [List.nodup_append]
-    simpa [p.2]⟩
-
-@[simp]
-lemma concat_val (p : G.Path x y) (h : G.IsBetween e y z) (hz : z ∉ p.vx) :
-  (concat p h hz).1 = p.1.concat h := rfl
-
-@[simp]
-lemma concat_vx (p : G.Path x y) (h : G.IsBetween e y z) (hz : z ∉ p.vx) :
-  (concat p h hz).vx = p.vx ++ [z] := by
-  simp [concat]
-
-@[simp]
-lemma concat_edge (p : G.Path x y) (h : G.IsBetween e y z) (hz : z ∉ p.vx) :
-  (concat p h hz).edge = p.edge ++ [e] := by
-  simp [concat]
-
-@[simp]
-lemma concat_length (p : G.Path x y) (h : G.IsBetween e y z) (hz : z ∉ p.vx) :
-  (concat p h hz).length = p.length + 1 := by
-  simp [concat]
-
-/-- Create a reversed path from one that goes from x to y to one from y to x -/
-def reverse (p : G.Path x y) : G.Path y x :=
-  ⟨p.1.reverse, by simp [Walk.reverse_vx]; exact p.2⟩
-
-@[simp]
-lemma reverse_val (p : G.Path x y) : (reverse p).1 = p.1.reverse := rfl
-
-@[simp]
-lemma reverse_vx (p : G.Path x y) : (reverse p).vx = p.vx.reverse := by
-  obtain ⟨W, hW⟩ := p
-  simp only [vx, reverse]
-  exact Walk.reverse_vx
-
-@[simp]
-lemma reverse_edge (p : G.Path x y) : (reverse p).edge = p.edge.reverse := by
-  obtain ⟨W, hW⟩ := p
-  simp only [edge, reverse]
-  exact Walk.reverse_edge
-
-@[simp]
-lemma reverse_length (p : G.Path x y) : (reverse p).length = p.length := by
-  obtain ⟨W, hW⟩ := p
-  simp only [length, reverse]
-  exact Walk.reverse_length
-
-def le {H : Graph α β} (p : G.Path x y) (hle : G ≤ H) : H.Path x y :=
-  ⟨p.1.le hle, by simp only [Walk.le_vx]; exact p.2⟩
-
-@[simp]
-lemma le_val (hle : G ≤ H) : (le p hle).1 = p.1.le hle := rfl
-
-@[simp]
-lemma le_vx (hle : G ≤ H) : (le p hle).vx = p.vx := by
-  simp [le, vx, Walk.le_vx]
-
-@[simp]
-lemma le_edge (hle : G ≤ H) : (le p hle).edge = p.edge := by
-  simp [le, edge, Walk.le_edge]
-
-@[simp]
-lemma le_length (hle : G ≤ H) : (le p hle).length = p.length := by
-  simp [le, length, Walk.le_length]
-
-def contract {α' : Type*} {f : α → α'} {C : Set β} (p : (G /[f] C).Path (f x) (f y)) : G.Path x y :=
-  sorry
+lemma nil_inj : (nil x : Path α β) = nil y ↔ x = y := by
+  rw [nil, nil, ← Subtype.val_inj, nil.injEq]
 
 end Path
 
--- def Walk.toPath [DecidableEq α] {x y : α} : G.Walk x y → G.Path x y := by
---   intro w
---   use w.dedup
---   sorry
+/-- Create a path from a single edge between two vertices -/
+def IsBetween.path (hbtw : G.IsBetween e u v) (hne : u ≠ v) : Path α β := ⟨hbtw.walk, by simp [hne]⟩
 
 namespace Path
+/-- Create the reverse of a path -/
+def reverse (p : Path α β) : Path α β := ⟨p.val.reverse, by simp [p.prop]⟩
 
-/-- Check if a path can be appended to another while maintaining the path property. -/
-def appendable (p₁ : G.Path x y) (p₂ : G.Path y z) : Prop :=
-  ∀ w, w ∈ p₁.vx.tail → w ∈ p₂.vx → w = y
+lemma ValidOn.le {p : Path α β} (h : p.ValidOn G) (hle : G ≤ H) : p.ValidOn H :=
+  Walk.ValidOn.le h hle
 
-/-- Append two paths if they can be appended while maintaining the path property. -/
-def append (p₁ : G.Path x y) (p₂ : G.Path y z) (h : appendable p₁ p₂) : G.Path x z := sorry
+lemma of_prefix {p : Path α β} {w1 w2 : Walk α β} (h : p.val = w1.append w2)
+    (heq : w1.finish = w2.start) : w1.vx.Nodup := by
+  have : (w1.append w2).vx = _ ++ _ := append_vx' heq
+  rw [← h] at this
+  have : w1.vx.Sublist p.val.vx := by
+    rw [this]
+    exact sublist_append_left w1.vx w2.vx.tail
+  exact this.nodup p.prop
 
--- @[simp]
--- lemma append_val (p₁ : G.Path x y) (p₂ : G.Path y z) (h : appendable p₁ p₂) :
---   (append p₁ p₂ h).1 = append p₁.1 p₂.1 (by simpa using h) := rfl
+lemma of_suffix {p : Path α β} {w1 w2 : Walk α β} (h : p.val = w1.append w2) : w2.vx.Nodup := by
+  have : (w1.append w2).vx = _ ++ w2.vx := append_vx
+  rw [← h] at this
+  have : w2.vx.Sublist p.val.vx := by
+    rw [this]
+    exact sublist_append_right w1.vx.dropLast w2.vx
+  exact this.nodup p.prop
 
-lemma append_vx (p₁ : G.Path x y) (p₂ : G.Path y z) (h : appendable p₁ p₂) :
-  (append p₁ p₂ h).vx = p₁.vx ++ p₂.vx.tail := sorry
+def append (p q : Path α β) (hDisj : p.vx.dropLast.Disjoint q.vx) : Path α β :=
+  ⟨p.val.append q.val, by
+    rw [append_vx]
+    refine List.Nodup.append ?_ q.prop hDisj
+    exact p.prop.sublist (List.dropLast_sublist p.vx)⟩
 
-lemma append_edge (p₁ : G.Path x y) (p₂ : G.Path y z) (h : appendable p₁ p₂) :
-  (append p₁ p₂ h).edge = p₁.edge ++ p₂.edge := sorry
+lemma edge_not_isLoop {p : Path α β} (he : e ∈ p.edge) (hVd : p.ValidOn G) : ¬ G.IsLoop e := by
+  intro hloop
+  rw [IsLoop_iff_IsBetween] at hloop
+  obtain ⟨x, hbtw⟩ := hloop
+  obtain ⟨w₁, w₂, hw12, hnin⟩ := eq_append_cons_of_edge_mem he
+  have hbtw' : G.IsBetween e w₁.finish w₂.start := by
+    simp only [ValidOn, hw12] at hVd
+    obtain ⟨hbtw, H2⟩ := hVd.append_right_validOn
+    exact hbtw
+  have hNodup := hw12 ▸ p.prop
+  simp only [append_vx, cons_vx] at hNodup
+  have := List.Nodup.of_append_right hNodup
+  obtain ⟨rfl, heq⟩ | ⟨rfl, heq⟩ := hbtw.eq_or_eq_of_IsBetween hbtw'
+  · rw [← w₂.vx.head_cons_tail vx_ne_nil, heq, start_eq_vx_head] at this
+    simp only [head_cons_tail, nodup_cons, head_mem, not_true_eq_false, false_and] at this
+  · rw [← w₂.vx.head_cons_tail vx_ne_nil, ← heq, start_eq_vx_head] at this
+    simp only [head_cons_tail, nodup_cons, head_mem, not_true_eq_false, false_and] at this
 
-lemma append_length (p₁ : G.Path x y) (p₂ : G.Path y z) (h : appendable p₁ p₂) :
-  (append p₁ p₂ h).length = p₁.length + p₂.length := sorry
+end Path
+
+@[simp]
+lemma IsBetween.path_vx (hbtw : G.IsBetween e u v) (hne : u ≠ v) :
+    (IsBetween.path hbtw hne).vx = [u, v] := by
+  simp only [Path.vx, path, Walk.vx]
+
+lemma Connected.iff_path : G.Connected u v ↔ ∃ p : Path α β, p.ValidOn G ∧ p.start = u ∧ p.finish = v := by
+  rw [Connected.iff_walk]
+  constructor
+  · rintro ⟨w, hwVd, rfl, rfl⟩
+    use Path.ofWalk w, dedup_validOn hwVd, dedup_start w, dedup_finish w
+  · rintro ⟨p, hpVd, rfl, rfl⟩
+    use p.val, hpVd, rfl
+    rfl
+
+lemma IsVxSetSeparator.path_inter {U : Set α} {S T : Set α} (hUsep : G.IsVxSetSeparator U S T)
+    (p : Path α β) (hVd : p.ValidOn G) (hS : p.start ∈ S) (hT : p.finish ∈ T) :
+    ∃ x ∈ p.vx, x ∈ U := by
+  by_contra! hx
+  have hVdU : p.ValidOn (G[G.V \ U]) := by
+    refine ValidOn.induce hVd ?_
+    rintro x hxp
+    exact ⟨hVd.mem_of_mem_vx hxp, hx x hxp⟩
+  exact hUsep p.val.start hS p.val.finish hT <| Walk.connected_of_validOn hVdU
+
+instance IsVxSetSeparator.IsPreorder {S : Set α} :
+    IsPreorder (Set α) (IsVxSetSeparator G · S ·) where
+  refl A := by
+    rintro s hs a ha hconn
+    have := hconn.mem_right
+    simp only [induce_V, mem_diff, ha, not_true_eq_false, and_false] at this
+  trans A B C hAB hBC := by
+    rintro s hs c hc hconn
+    rw [Connected.iff_path] at hconn
+    obtain ⟨p, hpVd, rfl, rfl⟩ := hconn
+    obtain ⟨x, hxp, hxB⟩ := hBC.path_inter p (hpVd.le (induce_le G Set.diff_subset)) hs hc
+    have := p.val.connected_of_validOn_of_mem hpVd start_vx_mem hxp
+    exact hAB p.val.start hs x hxB this
+
+lemma IsVxSetSeparator.crossingWalk_intersect {V S T : Set α} (h : G.IsVxSetSeparator V S T)
+    [DecidablePred (· ∈ V)] {w : Walk α β} (hwVd : w.ValidOn G) (hwstart : w.start ∈ h.leftSet ∪ V)
+    (hwfinish : w.finish ∈ h.rightSet ∪ V) : ∃ x ∈ w.vx, x ∈ V:= by
+  sorry
+
+lemma IsVxSetSeparator.crossingWalk_intersect' {V S T : Set α} (h : G.IsVxSetSeparator V S T)
+    [DecidablePred (· ∈ V)] {w : Walk α β} (hwVd : w.ValidOn G) (hwstart : w.start ∈ h.rightSet ∪ V)
+    (hwfinish : w.finish ∈ h.leftSet ∪ V) : ∃ x ∈ w.vx, x ∈ V:= by
+  sorry
+
+lemma IsVxSetSeparator.crossingWalk_endIf_validOn {V S T : Set α} (h : G.IsVxSetSeparator V S T)
+    [DecidablePred (· ∈ V)] (w : Walk α β) (hwVd : w.ValidOn G) (hwstart : w.start ∈ h.leftSet ∪ V)
+    (hwfinish : w.finish ∈ h.rightSet ∪ V) : (w.endIf (P := (· ∈ V))
+    (h.crossingWalk_intersect hwVd hwstart hwfinish)).ValidOn (G[h.leftSet ∪ V]) := by
+  sorry
+
+lemma IsVxSetSeparator.crossingWalk_endIf_validOn' {V S T : Set α} (h : G.IsVxSetSeparator V S T)
+    [DecidablePred (· ∈ V)] (w : Walk α β) (hwVd : w.ValidOn G) (hwstart : w.start ∈ h.rightSet ∪ V)
+    (hwfinish : w.finish ∈ h.leftSet ∪ V) : (w.endIf (P := (· ∈ V))
+    (h.crossingWalk_intersect' hwVd hwstart hwfinish)).ValidOn (G[h.rightSet ∪ V]) := by
+  sorry
+
+lemma IsVxSetSeparator.leftSetV_iff {V S T : Set α} (h : G.IsVxSetSeparator V S T) (hV : V ⊆ G.V)
+    (U : Set α) : G[h.leftSet ∪ V].IsVxSetSeparator U S V ↔ G.IsVxSetSeparator U S V := by
+  classical
+  constructor
+  · rintro hUsep s hs v hv hconn
+    rw [Connected.iff_walk] at hconn
+    obtain ⟨w, hwVd, rfl, rfl⟩ := hconn
+    have hwVdG : w.ValidOn G := hwVd.le (induce_le _ Set.diff_subset)
+    have hwstart : w.start ∈ h.leftSet ∪ V := by
+      by_cases hsUv : w.start ∈ V
+      · right
+        exact hsUv
+      · left
+        use w.start, hs
+        refine Connected.refl ⟨?_, hsUv⟩
+        exact Set.diff_subset <| hwVd.mem_of_mem_vx (Walk.start_vx_mem)
+    have hwfinish : w.finish ∈ h.rightSet ∪ V := Set.mem_union_right h.rightSet hv
+    have hw' : ∃ x ∈ w.vx, x ∈ V := h.crossingWalk_intersect hwVdG hwstart hwfinish
+    have := h.crossingWalk_endIf_validOn w hwVdG hwstart hwfinish
+    let w' := w.endIf (P := (· ∈ V)) hw'
+    apply hUsep w'.start (by rwa [Walk.endIf_start]) w'.finish (Walk.endIf_finish hw')
+    rw [induce_induce_eq_induce_right _ _ (Set.inter_subset_right.trans ?_), induce_V]
+    apply w'.connected_of_validOn
+    apply (Walk.endIf_validOn hw' hwVdG).induce
+    rintro x hx
+    exact ⟨this.mem_of_mem_vx hx, (hwVd.mem_of_mem_vx (Walk.endIf_vx_sublist hw' hx)).2⟩
+    · exact Set.diff_subset
+  · rintro hUsep
+    refine hUsep.le ?_
+    refine induce_le _ ?_
+    refine Set.union_subset ?_ ?_
+    · exact leftSet_subset h
+    · exact hV
+
+lemma IsVxSetSeparator.rightSetV_iff {V S T : Set α} (h : G.IsVxSetSeparator V S T) (hV : V ⊆ G.V)
+    (U : Set α) : G[h.rightSet ∪ V].IsVxSetSeparator U V T ↔ G.IsVxSetSeparator U V T := by
+  have := h.symm.leftSetV_iff hV U
+  rw [comm (S := V), comm (S := V)]
+  convert this using 1
+
+lemma IsVxSetSeparator.conn_sep_iff_conn_left {V S T : Set α} (h : G.IsVxSetSeparator V S T)
+    (hu : u ∈ h.leftSet) (hV : V ⊆ G.V) :
+    (∃ v ∈ V, G.Connected u v) ↔ ∃ v ∈ V, G[h.leftSet ∪ V].Connected u v := by
+  classical
+  constructor
+  · rintro ⟨v, hv, hconn⟩
+    rw [Connected.iff_walk] at hconn
+    obtain ⟨w, hwVd, rfl, rfl⟩ := hconn
+    have hw' : ∃ u ∈ w.vx, (fun x ↦ x ∈ V) u := by use w.finish, finish_vx_mem
+    let w' := w.endIf (P := (· ∈ V)) hw'
+    use w'.finish, Walk.endIf_finish hw'
+    rw [Connected.iff_walk]
+    use w', ?_, endIf_start hw'
+    have hw'VdG : w'.ValidOn G := endIf_validOn hw' hwVd
+    refine hw'VdG.induce ?_
+    rintro x hxw'
+    by_cases hNonempty : w'.Nonempty
+    · by_cases hxw'Finish : x = w'.finish
+      · subst x
+        right
+        exact endIf_finish hw'
+      · have hw'dVdG : w'.dropLast.ValidOn G := dropLast_validOn hw'VdG
+        have hw'dvdGV : w'.dropLast.ValidOn (G[G.V \ V]) := by
+          refine ValidOn.induce hw'dVdG ?_
+          rintro z hz
+          exact ⟨hw'dVdG.mem_of_mem_vx hz, endIf_dropLast_mem_vx hw' hNonempty hz⟩
+        have : w'.dropLast.ValidOn (G[h.leftSet]) := by
+          refine ValidOn.induce hw'dVdG ?_
+          rintro y hy
+          simp only [leftSet, mem_setOf_eq]
+          obtain ⟨s, hs, hsconn⟩ := hu
+          use s, hs
+          rw [← endIf_start hw', ← dropLast_start hNonempty] at hsconn
+          refine Connected.trans ?_ hsconn
+          exact w'.dropLast.connected_of_validOn_of_mem hw'dvdGV hy start_vx_mem
+
+        rw [← List.dropLast_concat_getLast vx_ne_nil, List.mem_append, ← dropLast_vx hNonempty,
+        List.mem_singleton, ← w'.finish_eq_vx_getLast] at hxw'
+        simp only [hxw'Finish, or_false] at hxw'
+        left
+        exact this.mem_of_mem_vx hxw'
+    · simp only [Nonempty.not_iff] at hNonempty
+      obtain ⟨y, hy⟩ := hNonempty
+      simp only [hy, nil_vx, mem_cons, not_mem_nil, or_false] at hxw'
+      subst y
+      right
+      have : w'.finish = x := by
+        simp only [hy, nil_finish]
+      exact this ▸ endIf_finish hw'
+  · rintro ⟨v, hv, hconn⟩
+    use v, hv
+    refine hconn.le (induce_le G ?_)
+    exact union_subset (h.leftSet_subset) hV
+
+lemma Contract.path {α' : Type*} {w : Walk α' β} {p : α → α'} {C : Set β} (hVd : ValidOn G p C)
+    (h : w.ValidOn (G /[p] C)) : ∀ x ∈ G.V, ∀ y ∈ G.V, p x = w.start → p y = w.finish →
+    ∃ w' : Path α β, w'.ValidOn G ∧ w'.start = x ∧ w'.finish = y ∧
+    {e | e ∈ w'.edge} ⊆ {e | e ∈ w.edge ∨ e ∈ C} := by
+  rintro x hx y hy hpx hpy
+  obtain ⟨w', hw'Vd, rfl, rfl, hsub⟩ := Contract.walk hVd h x hx y hy hpx hpy
+  use Path.ofWalk w', dedup_validOn hw'Vd, dedup_start w', dedup_finish w',
+    Subset.trans (dedup_edge_sublist w') hsub
 
 
+-- /-- If the endpoints of a path are connected in G via a valid path, they are connected in G -/
+-- lemma connected_of_validOn (h : p.ValidOn G u v) : G.Connected u v :=
+--   Walk.connected_of_validOn h
 
-
-/-- Paths establish connectivity between their endpoints. -/
-lemma connected (p : G.Path x y) : G.Connected x y :=
-  p.1.connected
-
--- /-- There is a path between two vertices if and only if they are connected. -/
--- lemma connected_iff : G.Connected x y ↔ Nonempty (G.Path x y) := by
---   constructor
---   · intro hConn
---     induction hConn with
---     | single hradj =>
---       expose_names
---       by_cases hxb : x = b
---       · subst b
---         use nil hradj.mem_left
---         simp
---       · have : G.Adj x b := by exact reflAdj.Adj_of_ne hradj hxb
-
-
-
---       use of_isBetween hradj hW.2
---     | tail hconn hradj ih =>
---       obtain ⟨W, hW⟩ := of_reflAdj hradj
---       use ih.some.append (of_isBetween hradj hW.2)
---       simpa using hW.1
-
---   · intro hPath
---     -- From path to connectivity: This direction is easy
---     exact hPath.some.connected
-
+namespace Path
 section disjoint
 
-variable {ι : Type*}
+/-- A collection of paths is internally disjoint if no vertex appears in more than one path
+  except for the special two vertices u and v. (i.e. the endpoints of the paths. But this is not
+  enforced in the definition) -/
+def InternallyDisjoint (u v : α) (Ps : Set (Path α β)) : Prop :=
+  ∀ x pi pj, pi ∈ Ps → pj ∈ Ps → x ∈ pi.vx → x ∈ pj.vx → pi ≠ pj → x = u ∨ x = v
 
-def InternallyDisjoint {G : Graph α β} {u v : α} (Ps : ι → G.Path u v) : Prop :=
-  ∀ i j x, x ∈ (Ps i).vx → x ∈ (Ps j).vx → i ≠ j → x = u ∨ x = v
+/-- A collection of paths is disjoint if no vertex appears in more than one path -/
+def Disjoint (Ps : Set (Path α β)) : Prop :=
+  ∀ x pi pj, pi ∈ Ps → pj ∈ Ps → x ∈ pi.vx → x ∈ pj.vx → pi = pj
 
-def Disjoint (u v : ι → α) (Ps : ∀ i, G.Path (u i) (v i)) : Prop :=
-  ∀ i j x, x ∈ (Ps i).vx → x ∈ (Ps j).vx → i = j
 
-theorem Menger {k : ℕ} (G : Graph α β) [G.Finite] (u v : α) (hu : u ∈ G.V) (hv : v ∈ G.V)
-    (huv : ¬ G.Adj u v) (h : ∀ S : Set α, S.Finite → G.IsVxSeparator u v S → k ≤ S.ncard) :
-    ∃ Ps : Fin k → G.Path u v, InternallyDisjoint Ps := by
-  classical
-  by_cases heuv : ∃ e : β, e ∈ G.E ∧ ¬ G.Inc u e ∧ ¬ G.Inc v e
-  · obtain ⟨e, he, hnuinc, hnvinc⟩ := heuv
-    have hG'le : G{G.E \ {e}} ≤ G := restrict_le G _
-    by_cases h :  ∀ (S : Set α), S.Finite → G{G.E \ {e}}.IsVxSeparator u v S → k ≤ S.ncard
-    · have hG'term : G{G.E \ {e}}.E.ncard < G.E.ncard := by
-        simp only [restrict_E]
-        apply Set.ncard_lt_ncard ?_ Finite.edge_fin
-        refine inter_ssubset_left_iff.mpr ?_
-        rintro hsu
-        have := hsu he
-        simp at this
-      have := Menger (G{G.E \ {e}}) u v hu hv (by contrapose! huv; exact huv.of_Adj_restrict ) h
-      obtain ⟨Ps, hPs⟩ := this
-      use fun i ↦ (Ps i).le hG'le
-      intro i j x hx hx' hne
-      refine hPs i j x ?_ ?_ hne
-      · simpa using hx
-      · simpa using hx'
-    · simp only [not_forall, Classical.not_imp, not_le] at h
-      obtain ⟨S, hSFin, hSsep, hcard⟩ := h
-      obtain ⟨x, y, hxy⟩ := G.exist_IsBetween_of_mem he
-      let G'' := G /[hxy.inc_left.contractFun] {e}
-      have hG''term : (G.E \ {e}).ncard < G.E.ncard := by
-        apply Set.ncard_lt_ncard ?_ Finite.edge_fin
-        simp [he]
-      have := Menger G'' u v (by sorry) (by sorry) (by sorry) sorry (k := k)
-      obtain ⟨Ps, hPs⟩ := this
-      obtain ⟨i, hi, hieq⟩ : ∃! i, x ∈ (Ps i).vx := by
-        sorry
-      sorry
-  · simp only [not_exists, not_and, not_not] at heuv
-    by_cases hadj : ∃ x : α, G.Adj u x ∧ G.Adj x v
-    · obtain ⟨x, hux, hxv⟩ := hadj
-      let G' := G[G.V \ {x}]
-      have hG'le : G' ≤ G := induce_le G Set.diff_subset
-      have hu' : u ∈ G'.V := by
-        simp only [induce_V, mem_diff, hu, mem_singleton_iff, true_and, G']
-        rintro rfl
-        exact huv hxv
-      have hv' : v ∈ G'.V := by
-        simp only [induce_V, mem_diff, hv, mem_singleton_iff, true_and, G']
-        rintro rfl
-        exact huv hux
-      have huv' : ¬ G'.Adj u v := by
-        contrapose! huv
-        exact huv.of_Adj_induce
-      have hG'Fin : G'.Finite := finite_of_le_finite hG'le
-      obtain ⟨eux, heux⟩ := hux
-      obtain ⟨exv, hexv⟩ := hxv
-      obtain p : G.Path u v := (of_isBetween hexv ?_).cons heux ?_
-      have hG'term : (G.E ∩ {e | ∀ (x_1 : α), G.Inc x_1 e → x_1 ∈ G.V ∧ ¬x_1 = x}).ncard + (k - 1) <
-        G.E.ncard + k := by sorry
-      have := Menger G' (k := k-1) u v hu' hv' huv' ?_
-      obtain ⟨Ps, hPs⟩ := this
+structure PathEnsemble (α β : Type*) [DecidableEq α] where
+  Paths : Set (Path α β)
+  Disj : Disjoint Paths
 
-      -- let Ps' : Fin k → G.Path u v := fun i ↦ Fin.cons sorry (fun i ↦ (Ps i).le hG'le) (i.cast (by sorry))
-      -- use Fin.cons sorry (fun i ↦ (Ps i).le hG'le)
-      sorry
-      sorry
-    · sorry
-termination_by G.E.ncard + k
+namespace PathEnsemble
 
+def Empty (α β : Type*) [DecidableEq α] : PathEnsemble α β where
+  Paths := ∅
+  Disj := by
+    rintro x p q hp hq hxp hxq
+    exact False.elim hp
+
+def nil (U : Set α) (β : Type*) : PathEnsemble α β where
+  Paths := Path.nil '' U
+  Disj := by
+    rintro x p q hp hq hxp hxq
+    simp only [mem_image] at hp hq
+    obtain ⟨u, hu, rfl⟩ := hp
+    obtain ⟨v, hv, rfl⟩ := hq
+    simp only [vx, Graph.Path.nil, nil_vx, mem_cons, not_mem_nil, or_false] at hxp hxq
+    subst u v
+    rfl
+
+def ValidOn (Ps : PathEnsemble α β) (G : Graph α β) := ∀ p ∈ Ps.Paths, p.ValidOn G
+
+def StartSet (Ps : PathEnsemble α β) : Set α := Path.start '' Ps.Paths
+
+def FinishSet (Ps : PathEnsemble α β) : Set α := Path.finish '' Ps.Paths
+
+def VxSet (Ps : PathEnsemble α β) : Set α := {x | ∃ p ∈ Ps.Paths, x ∈ p.vx}
+
+def EdgeSet (Ps : PathEnsemble α β) : Set β := {e | ∃ p ∈ Ps.Paths, e ∈ p.edge}
+
+def InternalVsSet (Ps : PathEnsemble α β) : Set α := {x | ∃ p ∈ Ps.Paths, x ∈ p.vx.tail.dropLast}
+
+def insert (p : Path α β) (Ps : PathEnsemble α β) (h : ∀ v ∈ p.vx, v ∉ Ps.VxSet) : PathEnsemble α β where
+  Paths := Ps.Paths ∪ {p}
+  Disj := by
+    rintro x p₁ p₂ hp1 hp2 hxp hxq
+    simp only [union_singleton, Set.mem_insert_iff] at hp1 hp2
+    simp only [VxSet, mem_setOf_eq, not_exists, not_and] at h
+    obtain (rfl | h1) := hp1 <;> obtain (rfl | h2) := hp2
+    · rfl
+    · exact (h x hxp p₂ h2 hxq).elim
+    · exact (h x hxq p₁ h1 hxp).elim
+    · exact Ps.Disj x p₁ p₂ h1 h2 hxp hxq
+
+@[simp]
+lemma Empty_validOn {G : Graph α β} : (Empty α β).ValidOn G := by
+  rintro p hp
+  exact False.elim hp
+
+@[simp]
+lemma Empty_finite : (Empty α β).Paths.Finite := by
+  simp only [Empty, finite_empty]
+
+@[simp]
+lemma Empty_ncard : (Empty α β).Paths.ncard = 0 := by
+  simp only [Empty, ncard_empty]
+
+@[simp]
+lemma Empty_VxSet : (Empty α β).VxSet = ∅ := by
+  simp only [VxSet, Empty, mem_empty_iff_false, false_and, exists_false, setOf_false]
+
+@[simp]
+lemma Empty_EdgeSet : (Empty α β).EdgeSet = ∅ := by
+  simp only [EdgeSet, Empty, mem_empty_iff_false, false_and, exists_false, setOf_false]
+
+@[simp]
+lemma Empty_startSet : (Empty α β).StartSet = ∅ := by
+  simp only [StartSet, Empty, image_empty]
+
+@[simp]
+lemma Empty_finishSet : (Empty α β).FinishSet = ∅ := by
+  simp only [FinishSet, Empty, image_empty]
+
+@[simp]
+lemma nil_validOn {U : Set α} {G : Graph α β} (hUV : U ⊆ G.V) : (nil U β).ValidOn G := by
+  rintro p hp
+  simp only [nil, ValidOn, mem_image] at hp
+  obtain ⟨q, hq, rfl⟩ := hp
+  exact hUV hq
+
+@[simp]
+lemma mem_nil_iff {U : Set α} {p : Path α β} : p ∈ (nil U β).Paths ↔ ∃ u ∈ U, Path.nil u = p := by
+  simp only [nil, mem_image]
+
+@[simp]
+lemma nil_VxSet {U : Set α} : (nil U β).VxSet = U := by
+  simp only [VxSet, mem_nil_iff, Path.nil, vx, exists_exists_and_eq_and, nil_vx, mem_cons,
+    not_mem_nil, or_false, exists_eq_right', setOf_mem_eq]
+
+@[simp]
+lemma nil_startSet {U : Set α} : (nil U β).StartSet = U := by
+  sorry
+
+@[simp]
+lemma nil_finishSet {U : Set α} : (nil U β).FinishSet = U := by
+  sorry
+
+@[simp]
+lemma nil_ncard {U : Set α} : (nil U β).Paths.ncard = U.ncard :=
+  ncard_image_of_injective U nil_injective
+
+lemma start_mem_StartSet {Ps : PathEnsemble α β} {p : Path α β} (hp : p ∈ Ps.Paths) :
+    p.start ∈ Ps.StartSet := by
+  use p, hp
+
+lemma finish_mem_FinishSet {Ps : PathEnsemble α β} {p : Path α β} (hp : p ∈ Ps.Paths) :
+    p.finish ∈ Ps.FinishSet := by
+  use p, hp
+
+lemma start_injOn (Ps : PathEnsemble α β) :
+    InjOn Path.start Ps.Paths := by
+  rintro p₁ hp₁ p₂ hp₂ hstart
+  exact Ps.Disj _ _ _ hp₁ hp₂ start_vx_mem (by
+    unfold Path.start at hstart
+    exact hstart ▸ start_vx_mem)
+
+lemma finish_injOn (Ps : PathEnsemble α β) :
+    InjOn Path.finish Ps.Paths := by
+  rintro p₁ hp₁ p₂ hp₂ hfinish
+  exact Ps.Disj _ _ _ hp₁ hp₂ finish_vx_mem (by
+    unfold Path.finish at hfinish
+    exact hfinish ▸ finish_vx_mem)
+
+lemma startSet_subset_VxSet {Ps : PathEnsemble α β} :
+    Ps.StartSet ⊆ Ps.VxSet := by
+  rintro x ⟨p, hp, rfl⟩
+  use p, hp, start_vx_mem
+
+lemma finishSet_subset_VxSet {Ps : PathEnsemble α β} :
+    Ps.FinishSet ⊆ Ps.VxSet := by
+  rintro x ⟨p, hp, rfl⟩
+  use p, hp, finish_vx_mem
+
+lemma VxSet_subset_of_validOn {Ps : PathEnsemble α β} (hVd : Ps.ValidOn G) : Ps.VxSet ⊆ G.V := by
+  rintro x ⟨p, hp, hx⟩
+  exact (hVd p hp).mem_of_mem_vx hx
+
+lemma StartSet_union_InternalVsSet (Ps : PathEnsemble α β) :
+    Ps.StartSet ∪ Ps.InternalVsSet = {x | ∃ p ∈ Ps.Paths, x ∈ p.vx.dropLast} := by
+  sorry
+
+lemma InternalVsSet_union_FinishSet (Ps : PathEnsemble α β) :
+    Ps.InternalVsSet ∪ Ps.FinishSet = {x | ∃ p ∈ Ps.Paths, x ∈ p.vx.tail} := by
+  sorry
+
+lemma StartSet_union_InternalVsSet_union_FinishSet (Ps : PathEnsemble α β) :
+    Ps.StartSet ∪ Ps.InternalVsSet ∪ Ps.FinishSet = Ps.VxSet := by
+  sorry
+
+lemma StartSet_InternalVsSet_disjoint (Ps : PathEnsemble α β) :
+    _root_.Disjoint Ps.StartSet Ps.InternalVsSet := by
+  sorry
+
+lemma StartSet_FinishSet_disjoint (Ps : PathEnsemble α β) :
+    _root_.Disjoint Ps.StartSet Ps.FinishSet := by
+  sorry
+
+lemma InternalVsSet_FinishSet_disjoint (Ps : PathEnsemble α β) :
+    _root_.Disjoint Ps.InternalVsSet Ps.FinishSet := by
+  sorry
+
+lemma VxSet_diff_StartSet (Ps : PathEnsemble α β) :
+    Ps.VxSet \ Ps.StartSet = Ps.InternalVsSet ∪ Ps.FinishSet := by
+  sorry
+
+lemma VxSet_diff_FinishSet (Ps : PathEnsemble α β) :
+    Ps.VxSet \ Ps.FinishSet = Ps.StartSet ∪ Ps.InternalVsSet := by
+  sorry
+
+lemma VxSet_diff_InternalVsSet (Ps : PathEnsemble α β) :
+    Ps.VxSet \ Ps.InternalVsSet = Ps.StartSet ∪ Ps.FinishSet := by
+  sorry
+
+lemma unique_path_start (Ps : PathEnsemble α β)  :
+    ∀ x ∈ Ps.StartSet, ∃! p ∈ Ps.Paths, p.start = x := by
+  rintro x hx
+  obtain ⟨p, hp, rfl⟩ := hx
+  use p, ⟨hp, rfl⟩
+  rintro q ⟨hq, hstart⟩
+  exact PathEnsemble.start_injOn Ps hq hp hstart
+
+lemma unique_path_finish (Ps : PathEnsemble α β) :
+    ∀ x ∈ Ps.FinishSet, ∃! p ∈ Ps.Paths, p.finish = x := by
+  rintro x hx
+  obtain ⟨p, hp, rfl⟩ := hx
+  use p, ⟨hp, rfl⟩
+  rintro q ⟨hq, hfinish⟩
+  exact PathEnsemble.finish_injOn Ps hq hp hfinish
+
+lemma StartSet_ncard {Ps : PathEnsemble α β} : Ps.StartSet.ncard = Ps.Paths.ncard := by
+  rw [eq_comm]
+  apply Set.ncard_congr (fun p hp ↦ Path.start p)
+  · rintro p hp
+    use p
+  · rintro p q hp hq hstart
+    exact Ps.Disj p.start p q hp hq start_vx_mem (hstart ▸ start_vx_mem)
+  · rintro x ⟨p, hp, rfl⟩
+    use p
+
+lemma FinishSet_ncard {Ps : PathEnsemble α β} : Ps.FinishSet.ncard = Ps.Paths.ncard := by
+  rw [eq_comm]
+  apply Set.ncard_congr (fun p hp ↦ Path.finish p)
+  · rintro p hp
+    use p
+  · rintro p q hp hq hfinish
+    exact Ps.Disj p.finish p q hp hq finish_vx_mem (hfinish ▸ finish_vx_mem)
+  · rintro x ⟨p, hp, rfl⟩
+    use p
+
+lemma ValidOn.le {Ps : PathEnsemble α β} {G G' : Graph α β} (h : G ≤ G') (hVd : Ps.ValidOn G) :
+    Ps.ValidOn G' := by
+  rintro p hp
+  exact (hVd p hp).le h
+
+lemma finite_of_finite_graph {Ps : PathEnsemble α β} {G : Graph α β} (h : G.Finite) (hVd : Ps.ValidOn G) :
+    Ps.Paths.Finite := by
+  have hle := (Ps.startSet_subset_VxSet).trans (Ps.VxSet_subset_of_validOn hVd)
+  have hst : Ps.StartSet.Finite := Finite.subset h.1 hle
+  exact (finite_image_iff Ps.start_injOn).mp hst
+
+@[simp]
+lemma mem_insert_iff {Ps : PathEnsemble α β} {p q : Path α β} (h : ∀ v ∈ p.vx, v ∉ Ps.VxSet) :
+    q ∈ (Ps.insert p h).Paths ↔ q = p ∨ q ∈ Ps.Paths := by
+  simp only [insert, union_singleton, Set.mem_insert_iff]
+
+lemma insert_validOn {Ps : PathEnsemble α β} {p : Path α β} (h : ∀ v ∈ p.vx, v ∉ Ps.VxSet)
+    (hVd : Ps.ValidOn G) (hpVd : p.ValidOn G) :
+    (Ps.insert p h).ValidOn G := by
+  rintro q hq
+  rw [mem_insert_iff] at hq
+  obtain (rfl | hq) := hq
+  · exact hpVd
+  · exact hVd q hq
+
+@[simp]
+lemma insert_ncard {Ps : PathEnsemble α β} {p : Path α β} (h : ∀ v ∈ p.vx, v ∉ Ps.VxSet)
+    (hFin : Ps.Paths.Finite) : (Ps.insert p h).Paths.ncard = Ps.Paths.ncard + 1 := by
+  simp [insert, VxSet] at h ⊢
+  apply Set.ncard_insert_of_not_mem ?_ hFin
+  rintro hp
+  obtain ⟨a, as, has⟩ := List.ne_nil_iff_exists_cons.mp (vx_ne_nil (w := p.val))
+  specialize h a (by simp [has, vx]) p hp
+  simp [has, vx] at h
+
+@[simp]
+lemma insert_startSet {Ps : PathEnsemble α β} {p : Path α β} (h : ∀ v ∈ p.vx, v ∉ Ps.VxSet) :
+    (Ps.insert p h).StartSet = Ps.StartSet ∪ {p.start} := by
+  simp only [StartSet, insert, union_singleton]
+  exact image_insert_eq
+
+@[simp]
+lemma insert_finishSet {Ps : PathEnsemble α β} {p : Path α β} (h : ∀ v ∈ p.vx, v ∉ Ps.VxSet) :
+    (Ps.insert p h).FinishSet = Ps.FinishSet ∪ {p.finish} := by
+  simp only [FinishSet, insert, union_singleton]
+  exact image_insert_eq
+
+def append (Ps₁ Ps₂ : PathEnsemble α β) (h₁Finish : Ps₁.VxSet ∩ Ps₂.VxSet = Ps₁.FinishSet)
+    (h₂Start : Ps₁.VxSet ∩ Ps₂.VxSet = Ps₂.StartSet) : PathEnsemble α β where
+  Paths := by
+    let f : ↑(Ps₁.VxSet ∩ Ps₂.VxSet) → Path α β := fun ⟨a, ha⟩ ↦
+      (Ps₁.unique_path_finish a (h₁Finish ▸ ha)).choose.append
+      (Ps₂.unique_path_start a (h₂Start ▸ ha)).choose ?_
+    exact Set.range f
+    · rintro b hbf hbg
+      have h : b ∈ {x | ∃ p ∈ Ps₁.Paths, x ∈ p.vx.dropLast} := by
+        use (Ps₁.unique_path_finish a (h₁Finish ▸ ha)).choose, (Ps₁.unique_path_finish a (h₁Finish ▸ ha)).choose_spec.1.1
+      rw [← StartSet_union_InternalVsSet, ← VxSet_diff_FinishSet, ← h₁Finish, Set.diff_self_inter] at h
+      obtain ⟨H1, H2⟩ := h
+      have hb2 : b ∈ Ps₂.VxSet := by
+        use (Ps₂.unique_path_start a (h₂Start ▸ ha)).choose, (Ps₂.unique_path_start a (h₂Start ▸ ha)).choose_spec.1.1
+      exact H2 hb2
+  Disj := by
+    rintro x p q hp hq hxp hxq
+    rw [Set.mem_range, Subtype.exists] at hp hq
+    obtain ⟨a, ha, rfl⟩ := hp
+    obtain ⟨b, hb, rfl⟩ := hq
+    have hw1a := (Ps₁.unique_path_finish a (h₁Finish ▸ ha)).choose_spec
+    have hw2a := (Ps₂.unique_path_start a (h₂Start ▸ ha)).choose_spec
+    have hw1b := (Ps₁.unique_path_finish b (h₁Finish ▸ hb)).choose_spec
+    have hw2b := (Ps₂.unique_path_start b (h₂Start ▸ hb)).choose_spec
+    simp only [vx, Path.append, append_vx, mem_append] at hxp hxq
+    suffices h : a = b by
+      subst b
+      rfl
+    obtain (hxp1 | hxp2) := hxp <;> obtain (hxq1 | hxq2) := hxq
+    · have := Ps₁.Disj x _ _ hw1a.1.1 hw1b.1.1 (List.dropLast_subset _ hxp1) (List.dropLast_subset _ hxq1)
+      rw [← hw1a.1.2, ← hw1b.1.2, this]
+    · have h1 : x ∈ {x | ∃ p ∈ Ps₁.Paths, x ∈ p.vx.dropLast} := by
+        use (Ps₁.unique_path_finish a (h₁Finish ▸ ha)).choose, hw1a.1.1, hxp1
+      rw [← StartSet_union_InternalVsSet, ← VxSet_diff_FinishSet, ← h₁Finish, Set.diff_self_inter] at h1
+      obtain ⟨H1, H2⟩ := h1
+      have h2 : x ∈ Ps₂.VxSet := by
+        use (Ps₂.unique_path_start b (h₂Start ▸ hb)).choose, hw2b.1.1, hxq2
+      exact False.elim (H2 h2)
+    · have h1 : x ∈ {x | ∃ p ∈ Ps₁.Paths, x ∈ p.vx.dropLast} := by
+        use (Ps₁.unique_path_finish b (h₁Finish ▸ hb)).choose, hw1b.1.1, hxq1
+      rw [← StartSet_union_InternalVsSet, ← VxSet_diff_FinishSet, ← h₁Finish, Set.diff_self_inter] at h1
+      obtain ⟨H1, H2⟩ := h1
+      have h2 : x ∈ Ps₂.VxSet := by
+        use (Ps₂.unique_path_start a (h₂Start ▸ ha)).choose, hw2a.1.1, hxp2
+      exact False.elim (H2 h2)
+    · have := Ps₂.Disj x _ _ hw2a.1.1 hw2b.1.1 hxp2 hxq2
+      rw [← hw2a.1.2, ← hw2b.1.2, this]
+
+
+  -- Paths := by
+  --   let f : Ps₁.Paths → Path α β := fun ⟨p, hp⟩ ↦ p.append (h p hp).choose ?_
+  --   exact Set.range f
+  --   rintro a hap haq
+  --   obtain ⟨hmem2, hstart⟩ := (h p hp).choose_spec
+  --   have haG := (hPs₁Vd p hp).mem_of_mem_vx (List.dropLast_subset p.vx hap)
+  --   have haH := (hPs₂Vd (h p hp).choose hmem2).mem_of_mem_vx haq
+  --   have hVxDisj := vx_disjoint_of_disjoint hGH (by simp [haG] : {a} ≤ _) (by simp [haH] : {a} ≤ _)
+  --   simp only [bot_eq_empty, le_eq_subset, subset_empty_iff, singleton_ne_empty] at hVxDisj
+  -- Disj := by
+  --   rintro x p q hp hq hxp hxq
+  --   simp only [Set.mem_range, Subtype.exists] at hp hq
+  --   obtain ⟨w1, hw1, rfl⟩ := hp
+  --   obtain ⟨w2, hw2, rfl⟩ := hq
+  --   simp only [vx, Graph.Path.append, append_vx, mem_append] at hxp hxq
+  --   suffices hw12 : w1 = w2 by
+  --     subst w2
+  --     rfl
+  --   obtain (hxp1 | hxp2) := hxp <;> obtain (hxq1 | hxq2) := hxq
+  --   · exact Ps₁.Disj _ _ _ hw1 hw2 (List.dropLast_subset w1.vx hxp1) (List.dropLast_subset w2.vx hxq1)
+  --   · obtain ⟨hmem2, hstart⟩ := (h w2 hw2).choose_spec
+  --     have haG := (hPs₁Vd w1 hw1).mem_of_mem_vx (List.dropLast_subset w1.vx hxp1)
+  --     have haH := (hPs₂Vd (h w2 hw2).choose hmem2).mem_of_mem_vx hxq2
+  --     have hVxDisj := vx_disjoint_of_disjoint hGH (by simp [haG] : {x} ≤ _) (by simp [haH] : {x} ≤ _)
+  --     simp only [bot_eq_empty, le_eq_subset, subset_empty_iff, singleton_ne_empty] at hVxDisj
+  --   · obtain ⟨hmem1, hstart⟩ := (h w1 hw1).choose_spec
+  --     have haG := (hPs₁Vd w2 hw2).mem_of_mem_vx (List.dropLast_subset w2.vx hxq1)
+  --     have haH := (hPs₂Vd (h w1 hw1).choose hmem1).mem_of_mem_vx hxp2
+  --     have hVxDisj := vx_disjoint_of_disjoint hGH (by simp [haG] : {x} ≤ _) (by simp [haH] : {x} ≤ _)
+  --     simp only [bot_eq_empty, le_eq_subset, subset_empty_iff, singleton_ne_empty] at hVxDisj
+  --   · obtain ⟨hmem1, hstart1⟩ := (h w1 hw1).choose_spec
+  --     obtain ⟨hmem2, hstart2⟩ := (h w2 hw2).choose_spec
+  --     have := Ps₂.Disj _ _ _ hmem1 hmem2 hxp2 hxq2
+  --     change (h w1 hw1).choose = (h w2 hw2).choose at this
+  --     apply Ps₁.Disj _ _ _ hw1 hw2 finish_vx_mem
+  --     unfold Path.finish at hstart1 hstart2
+  --     rw [hstart1, this, ← hstart2]
+  --     exact finish_vx_mem
+
+lemma append_validOn {G : Graph α β} {Ps₁ Ps₂ : PathEnsemble α β}
+    (hPs₁Vd : Ps₁.ValidOn G) (hPs₂Vd : Ps₂.ValidOn G) (h₁Finish : Ps₁.VxSet ∩ Ps₂.VxSet = Ps₁.FinishSet)
+    (h₂Start : Ps₁.VxSet ∩ Ps₂.VxSet = Ps₂.StartSet) : (Ps₁.append Ps₂ h₁Finish h₂Start).ValidOn G := by
+  rintro p hp
+  obtain ⟨⟨a, ha⟩, _, rfl⟩ := hp
+  unfold Path.append Path.ValidOn
+  let w1 := (Ps₁.unique_path_finish a (h₁Finish ▸ ha)).choose
+  let w2 := (Ps₂.unique_path_start a (h₂Start ▸ ha)).choose
+  have hw1a := (Ps₁.unique_path_finish a (h₁Finish ▸ ha)).choose_spec
+  have hw2a := (Ps₂.unique_path_start a (h₂Start ▸ ha)).choose_spec
+  change (w1.val.append w2.val).ValidOn G
+  apply Walk.append_validOn
+  · exact hw1a.1.2.trans hw2a.1.2.symm
+  · exact hPs₁Vd _ hw1a.1.1
+  · exact hPs₂Vd _ hw2a.1.1
+
+lemma append_ncard_eq_left {Ps₁ Ps₂ : PathEnsemble α β} (h₁Finish : Ps₁.VxSet ∩ Ps₂.VxSet = Ps₁.FinishSet)
+    (h₂Start : Ps₁.VxSet ∩ Ps₂.VxSet = Ps₂.StartSet) (hFin : Ps₁.Paths.Finite) :
+    (Ps₁.append Ps₂ h₁Finish h₂Start).Paths.ncard = Ps₁.Paths.ncard := by
+  sorry
+
+lemma append_ncard_eq_right {Ps₁ Ps₂ : PathEnsemble α β} (h₁Finish : Ps₁.VxSet ∩ Ps₂.VxSet = Ps₁.FinishSet)
+    (h₂Start : Ps₁.VxSet ∩ Ps₂.VxSet = Ps₂.StartSet) (hFin : Ps₂.Paths.Finite) :
+    (Ps₁.append Ps₂ h₁Finish h₂Start).Paths.ncard = Ps₂.Paths.ncard := by
+  sorry
+
+lemma append_startSet {Ps₁ Ps₂ : PathEnsemble α β} (h₁Finish : Ps₁.VxSet ∩ Ps₂.VxSet = Ps₁.FinishSet)
+    (h₂Start : Ps₁.VxSet ∩ Ps₂.VxSet = Ps₂.StartSet) :
+    (Ps₁.append Ps₂ h₁Finish h₂Start).StartSet = Ps₁.StartSet := by
+  sorry
+
+lemma append_finishSet {Ps₁ Ps₂ : PathEnsemble α β} (h₁Finish : Ps₁.VxSet ∩ Ps₂.VxSet = Ps₁.FinishSet)
+    (h₂Start : Ps₁.VxSet ∩ Ps₂.VxSet = Ps₂.StartSet) :
+    (Ps₁.append Ps₂ h₁Finish h₂Start).FinishSet = Ps₂.FinishSet := by
+  sorry
+
+lemma append_VxSet {Ps₁ Ps₂ : PathEnsemble α β} (h₁Finish : Ps₁.VxSet ∩ Ps₂.VxSet = Ps₁.FinishSet)
+    (h₂Start : Ps₁.VxSet ∩ Ps₂.VxSet = Ps₂.StartSet) :
+    (Ps₁.append Ps₂ h₁Finish h₂Start).VxSet = Ps₁.VxSet ∪ Ps₂.VxSet := by
+  sorry
+
+end PathEnsemble
 
 end disjoint
 
 end Path
-
-
-
-
--- end Path
