Kura/Menger.lean
@@ -1,4 +1,4 @@
-import Kura.Walk2
+import Kura.Walk
 
 open Set Function List Nat
 variable {α β : Type*} {G H : Graph α β} {u v x y z : α} {e e' f g : β}
@@ -30,48 +30,44 @@ theorem Menger_VxSet {α β : Type*} [DecidableEq α] (G : Graph α β) [hfin : 
       use Ps, hlen, fun p hp ↦ (hPVd p hp).le hG'le
     · simp only [not_forall, Classical.not_imp, not_le] at h
       obtain ⟨U, hUFin, hUsep, hUcard⟩ := h
-      have hUcard' : U.ncard = k -1 := by sorry -- TODO: deal with k = 0 case
-      have hUV : U ⊆ G.V := by sorry
 
       -- There is a path that uses e and none of the vertices in U
-      -- TODO: Just use Connected.exists_walk?
-      have hterm : (G.E ∩ {e | ∀ (x : α), G.Inc x e → x ∈ G.V ∧ x ∉ U}).ncard + 1 < G.E.ncard + k := by
-        have : (G.E ∩ {e | ∀ (x : α), G.Inc x e → x ∈ G.V ∧ x ∉ U}).ncard ≤ G.E.ncard :=
-          Set.ncard_inter_le_ncard_left G.E _ hfin.edge_fin
-        suffices 1 < k by
-          omega
-        sorry -- TODO: deal with k = 1 case too
-      obtain ⟨Ps, hlen, hPVd, hPsStart, hPsFinish⟩ := Menger_VxSet (hfin := finite_of_finite_induce hfin.vx_fin.diff)
-        (G[G.V \ U]) S T 1 hS hT (by
-        rintro V hVFin hVsep
-        by_contra! hVcard
-        simp only [lt_one_iff, hVFin, ncard_eq_zero] at hVcard
-        subst V
-        simp only [IsVxSetSeparator, induce_V, diff_empty, induce_idem] at hVsep
-        have := hsep U hUFin hVsep
-        omega)
-      simp only [ncard_eq_one] at hlen
-      obtain ⟨p, hp⟩ := hlen
-      simp only [PathEnsemble.ValidOn, hp, mem_singleton_iff, forall_eq] at hPVd
-      have hpmem : p ∈ Ps.Paths := by simp only [hp, mem_singleton_iff]
+      have : ¬ G.IsVxSetSeparator U S T := by
+        rintro h
+        specialize hsep U hUFin h
+        omega
+      simp only [IsVxSetSeparator, not_forall, Classical.not_imp, Decidable.not_not] at this
+      obtain ⟨s, hs, t, ht, hconn⟩ := this
+      rw [Connected.iff_path] at hconn
+      obtain ⟨p, hpVdU, rfl, rfl⟩ := hconn
+      have hpVd : p.ValidOn G := hpVdU.le (induce_le G Set.diff_subset)
       have hpe : e ∈ p.edge := by
         by_contra! hpe
-        refine hUsep p.start (hPsStart (Ps.start_mem_StartSet hpmem)) p.finish
-          (hPsFinish (Ps.finish_mem_FinishSet hpmem)) (Walk.connected_of_validOn ?_)
-        have := Walk.ValidOn.restrict hPVd (?_ : ∀ f ∈ p.edge, f ∈ G.E \ {e})
-        simpa only [restrict_V, induce_restrict_eq_subgraph] using this
-        · rintro f hf
-          refine ⟨Set.mem_of_mem_inter_left (Walk.ValidOn.mem_of_mem_edge hPVd hf), ?_⟩
-          rw [mem_singleton_iff]
+        apply hUsep p.start hs p.finish ht
+        rw [restrict_V]
+        apply p.val.connected_of_validOn
+        apply hpVd.subgraph
+        · rintro x hx
+          exact hpVdU.mem_of_mem_vx hx
+        · rintro e' he'
+          refine ⟨hpVd.mem_of_mem_edge he', ?_⟩
+          simp only [mem_singleton_iff]
           rintro rfl
-          exact hpe hf
-
+          exact hpe he'
       obtain ⟨w₁, w₂, hw12, hnin⟩ := Walk.eq_append_cons_of_edge_mem hpe
+      have hw₁start : w₁.start = p.start := by
+        unfold Path.start
+        rw [hw12]
+        simp only [Walk.cons_start, Walk.append_start_of_eq]
+      have hw₂finish : w₂.finish = p.finish := by
+        unfold Path.finish
+        rw [hw12]
+        simp only [Walk.append_finish, Walk.cons_finish]
       let x := w₁.finish
       let y := w₂.start
       have hxy : G[G.V \ U].IsBetween e x y := by
-        simp only [ValidOn, hw12] at hPVd
-        obtain ⟨hbtw, H2⟩ := hPVd.append_right_validOn
+        simp only [ValidOn, hw12] at hpVdU
+        obtain ⟨hbtw, H2⟩ := hpVdU.append_right_validOn
         exact hbtw
       have hxney : x ≠ y := by
         rintro hxeqy
@@ -79,92 +75,170 @@ theorem Menger_VxSet {α β : Type*} [DecidableEq α] (G : Graph α β) [hfin : 
         have hloop : G[G.V \ U].IsLoop e := by
           rw [IsLoop_iff_IsBetween]
           use y
-        exact edge_not_isLoop hpe hPVd hloop
-
-      /- TODO: U is a separator on G - e. If U contains either x or y, then removing U from G also removes
-      the edge e. This implies that U is also a separator of G. As U is smaller than k, this is a
-      contradiction. -/
-      have hxU : x ∉ U := by sorry
-      have hyU : y ∉ U := by sorry
-
-      let PU : PathEnsemble α β := {
-        Paths := insert (IsBetween.path hxy hxney) (Path.nil '' U)
-        Disj := by
-          rintro z p q hp hq hzp hzq
-          simp only [Set.mem_insert_iff, mem_image] at hp hq
-          obtain rfl | ⟨z', hz', rfl⟩ := hp <;> obtain rfl | ⟨z'', hz'', rfl⟩ := hq
-          · rfl
-          · simp only [vx, nil, Walk.nil_vx, mem_cons, not_mem_nil, or_false, IsBetween.path,
-            IsBetween.Walk.vx] at hzq hzp
-            subst z''
-            obtain rfl | rfl := hzp
-            · exact False.elim (hxU hz'')
-            · exact False.elim (hyU hz'')
-          · simp only [vx, nil, Walk.nil_vx, mem_cons, not_mem_nil, or_false, IsBetween.path,
-            IsBetween.Walk.vx] at hzq hzp
-            subst z'
-            obtain rfl | rfl := hzq
-            · exact False.elim (hxU hz')
-            · exact False.elim (hyU hz')
-          · simp only [vx, nil, Walk.nil_vx, mem_cons, not_mem_nil, or_false] at hzp hzq
-            subst z' z''
-            rfl
-      }
-
-      have hterm : (G.E ∩ (G.E \ {e})).ncard < G.E.ncard := by
-        refine lt_of_le_of_lt (Set.ncard_inter_le_ncard_right G.E _ hfin.edge_fin.diff) ?_
-        rw [Set.ncard_diff (by simp only [singleton_subset_iff, he])]
-        simp only [ncard_singleton, tsub_lt_self_iff, lt_one_iff, pos_of_gt, and_true]
-        rw [Set.ncard_pos hfin.edge_fin]
-        exact nonempty_of_mem he
+        exact edge_not_isLoop hpe hpVdU hloop
 
       let Ux := U ∪ {x}
+      have hUxconn : G[G.V \ Ux].Connected y p.finish := by
+        rw [← hw₂finish]
+        refine w₂.connected_of_validOn ?_
+        unfold Path.ValidOn at hpVdU
+        rw [hw12] at hpVdU
+        have := hpVdU.append_right_validOn
+        rw [Walk.cons_validOn_iff] at this
+        have h2Vd := this.2.le (induce_le G Set.diff_subset)
+        refine Walk.ValidOn.induce h2Vd ?_
+        rintro z hz2
+        refine ⟨h2Vd.mem_of_mem_vx hz2, ?_⟩
+        simp only [union_singleton, Set.mem_insert_iff, (this.2.mem_of_mem_vx hz2).2, or_false, Ux]
+        rintro rfl
+        have := p.prop
+        rw [hw12] at this
+        simp only [Walk.append_vx, Walk.cons_vx] at this
+        exact List.not_nodup_cons_of_mem hz2 <| List.Nodup.of_append_right this
+      have hUxFin : Ux.Finite := hUFin.union (finite_singleton x)
+      have hUxSep : G.IsVxSetSeparator Ux S T := by
+        rintro a ha b hb hconn
+        refine hUsep a ha b hb (hconn.le ?_)
+        simp only [restrict_V]
+        rw [le_of_exist_mutual_le]
+        refine ⟨?_, ?_⟩
+        · simp only [union_singleton, induce_V, Ux]
+          rw [Set.diff_subset_comm]
+          simp only [sdiff_sdiff_right_self, inf_eq_inter]
+          exact Set.inter_subset_right.trans (Set.subset_insert x U)
+        · rintro f
+          simp +contextual only [union_singleton, induce_E, mem_diff, Set.mem_insert_iff, not_or,
+            Set.mem_inter_iff, mem_setOf_eq, restrict_E, restrict_inc, mem_singleton_iff, and_imp,
+            true_and, not_false_eq_true, and_self, implies_true, imp_self, and_true, Ux, x]
+          rintro hf hf' rfl
+          specialize hf' x (hxy.le (induce_le G Set.diff_subset)).inc_left
+          simp only [not_true_eq_false, false_and, and_false, x, Ux] at hf'
+        · exact induce_le G Set.diff_subset
+        · exact (induce_le _ Set.diff_subset).trans (restrict_le G _)
+      have hUxncard : Ux.ncard = k := by
+        specialize hsep Ux hUxFin hUxSep
+        have : Ux.ncard ≤ U.ncard + 1 := by
+          simp only [union_singleton, Ux]
+          exact ncard_insert_le x U
+        omega
+      have hxU : x ∉ U := by
+        rintro hxU
+        simp only [union_singleton, hxU, insert_eq_of_mem, Ux] at hUxncard
+        omega
+      let Uy := U ∪ {y}
+      have hUyconn : G[G.V \ Uy].Connected p.start x := by
+        rw [← hw₁start]
+        refine w₁.connected_of_validOn ?_
+        unfold Path.ValidOn at hpVdU
+        rw [hw12] at hpVdU
+        by_cases h : w₁.Nonempty
+        · have := hpVdU.append_left_validOn (by simp) h
+          have h1Vd := this.le (induce_le G Set.diff_subset)
+          refine Walk.ValidOn.induce h1Vd ?_
+          rintro z hz2
+          refine ⟨h1Vd.mem_of_mem_vx hz2, ?_⟩
+          simp only [union_singleton, Set.mem_insert_iff, (this.mem_of_mem_vx hz2).2, or_false, Uy]
+          rintro rfl
+          have := p.prop
+          rw [hw12] at this
+          simp only [Walk.append_vx, Walk.cons_vx] at this
+          rw [List.append_cons, Walk.finish_eq_vx_getLast, List.dropLast_concat_getLast Walk.vx_ne_nil] at this
+          exact List.disjoint_of_nodup_append this hz2 Walk.start_vx_mem
+        · simp only [Walk.Nonempty.not_iff, Uy] at h
+          obtain ⟨u, rfl⟩ := h
+          simp only [Walk.nil_validOn_iff, induce_V, mem_diff, Uy]
+          have : x = u := by
+            unfold x
+            rfl
+          rw [this] at hxU hxney hxy
+          refine ⟨diff_subset hxy.vx_mem_left, ?_⟩
+          simp only [union_singleton, Set.mem_insert_iff, hxney, hxU, or_self, not_false_eq_true]
+
+      have hUyFin : Uy.Finite := hUFin.union (finite_singleton y)
+      have hUySep : G.IsVxSetSeparator Uy S T := by
+        rintro a ha b hb hconn
+        refine hUsep a ha b hb (hconn.le ?_)
+        simp only [restrict_V]
+        rw [le_of_exist_mutual_le]
+        refine ⟨?_, ?_⟩
+        · simp only [union_singleton, induce_V, Uy]
+          rw [Set.diff_subset_comm]
+          simp only [sdiff_sdiff_right_self, inf_eq_inter]
+          exact Set.inter_subset_right.trans (Set.subset_insert y U)
+        · rintro f
+          simp +contextual only [union_singleton, induce_E, mem_diff, Set.mem_insert_iff, not_or,
+            Set.mem_inter_iff, mem_setOf_eq, restrict_E, restrict_inc, mem_singleton_iff, and_imp,
+            true_and, not_false_eq_true, and_self, implies_true, imp_self, and_true, Uy, y]
+          rintro hf hf' rfl
+          specialize hf' y (hxy.le (induce_le G Set.diff_subset)).inc_right
+          simp only [not_true_eq_false, false_and, and_false, y, Uy] at hf'
+        · exact induce_le G Set.diff_subset
+        · exact (induce_le _ Set.diff_subset).trans (restrict_le G _)
+      have hUyncard : Uy.ncard = k := by
+        specialize hsep Uy hUyFin hUySep
+        have : Uy.ncard ≤ U.ncard + 1 := by
+          simp only [union_singleton, Uy]
+          exact ncard_insert_le y U
+        omega
+      have hyU : y ∉ U := by
+        rintro hyU
+        simp only [union_singleton, hyU, insert_eq_of_mem, Uy] at hUyncard
+        omega
+      have hUV : U ⊆ G.V := by
+        change ∀ x ∈ U, x ∈ G.V
+        by_contra! hUV
+        obtain ⟨u, huU, huv⟩ := hUV
+        have hUdiffu : (Ux \ {u}).ncard < Ux.ncard := by
+          refine Set.ncard_lt_ncard ?_ hUxFin
+          simp only [union_singleton, diff_ssubset_left_iff, inter_singleton_nonempty,
+            Set.mem_insert_iff, huU, or_true, Ux, x, Uy, y]
+        specialize hsep (Ux \ {u}) (Finite.diff hUxFin) ?_
+        · rintro a ha b hb hconn
+          refine hUxSep a ha b hb ?_
+          convert hconn using 2
+          rw [Set.diff_diff_right, eq_comm, Set.union_eq_left, Set.inter_singleton_eq_empty.mpr huv]
+          exact empty_subset (G.V \ Ux)
+        omega
       have hUx : Ux ⊆ G.V := by
         simp [Ux, hUV, Set.insert_subset_iff, (Set.diff_subset hxy.vx_mem_left)]
-      let L : Set α := {l | ∃ s ∈ S, G[G.V \ Ux].Connected l s}
+      have hUy : Uy ⊆ G.V := by
+        simp [Uy, hUV, Set.insert_subset_iff, (Set.diff_subset hxy.vx_mem_right)]
+
+      let PU : PathEnsemble α β := PathEnsemble.insert (hxy.path hxney) (PathEnsemble.nil U β) (by
+        rintro z hz
+        simp only [hxy.path_vx, mem_cons, not_mem_nil, or_false] at hz
+        obtain rfl | rfl := hz <;> simp only [PathEnsemble.nil_VxSet, hxU, hyU, not_false_eq_true])
+      have hxyVdG : (hxy.path hxney).ValidOn G := hxy.walk_validOn.le (induce_le G Set.diff_subset)
+      have hPUVdUxy : PU.ValidOn (G[insert x (insert y U)]) := by
+        rintro p (hp | hp)
+        · simp only [PathEnsemble.mem_nil_iff, nil] at hp
+          obtain ⟨u, hu, rfl⟩ := hp
+          simp only [ValidOn, Walk.nil_validOn_iff, induce_V, Set.mem_insert_iff, hu, or_true]
+        · rw [mem_singleton_iff] at hp
+          subst p
+          simp only [ValidOn]
+          refine Walk.ValidOn.induce hxyVdG ?_
+          rintro a ha
+          simp only [IsBetween.path, IsBetween.Walk.vx, mem_cons, not_mem_nil, or_false] at ha
+          obtain rfl | rfl := ha <;> simp
+
+      let L : Set α := hUxSep.leftSet
+      let R : Set α := hUySep.rightSet
+      have hLy : y ∉ L := by
+        rintro ⟨s, hs, hconn⟩
+        exact hUxSep s hs p.finish ht <| hconn.symm.trans hUxconn
+      have hRx : x ∉ R := by
+        rintro ⟨t, ht, hconn⟩
+        exact hUySep p.start hs t ht <| hUyconn.trans hconn
+
       have hLV : L ⊆ G.V := by
         rintro l ⟨s, hs, hconn⟩
         exact Set.diff_subset hconn.mem_left
-      have hUxFin : Ux.Finite := hUFin.union (finite_singleton x)
-      have hUxncard : Ux.ncard = k := by sorry
-      -- TODO: U is a separator on G - e. Then, G \ Ux ≤ (G - e) \ U. Connected.le
-      have hUxSep : G.IsVxSetSeparator Ux S T := by
-        sorry
-      -- ...
       have hSUxSepCard : ∀ (U : Set α), U.Finite → G[L ∪ Ux].IsVxSetSeparator U S Ux → k ≤ U.ncard := by
         rintro V hVFin hVsep
-        refine hsep V hVFin ?_
-        rintro a ha b hb hconn
-        obtain ⟨p, hpVd, rfl, rfl⟩ := Connected.iff_path.mp hconn
-        have hexists : ∃ u ∈ p.val.vx, u ∉ L := by
-          use p.val.finish, Walk.finish_vx_mem
-          simp only [mem_setOf_eq, not_exists, not_and, L]
-          rintro s hs h
-          exact hUxSep s hs p.finish hb h.symm
-        let w := p.val.endIf (P := fun x ↦ x ∉ L) hexists
-        have hp'start : w.start = p.start := Walk.endIf_start _
-        have hp'finish : w.finish ∈ Ux := by
-          obtain ⟨z, hzw, hzL, f, hbtw⟩ := Walk.endIf_exists_isBetween_last hexists hpVd sorry -- TODO: w has at least 2 vertices hence nonempty
-          have : w.finish ∉ L := Walk.endIf_finish hexists
-          simp only [mem_setOf_eq, not_exists, not_forall, Decidable.not_not, L] at hzL this
-          simp_rw [not_and] at this
-          exact foo (hbtw.le (induce_le G Set.diff_subset)) hzL this
-        have hp'Vd1 : w.ValidOn (G[G.V \ V]) := Walk.endIf_validOn _ hpVd
-        have hp'Vd : w.ValidOn (G[(L ∪ Ux) \ V]) := by
-          refine Walk.ValidOn.induce (hp'Vd1.le (induce_le G Set.diff_subset)) ?_
-          rintro x hx
-          refine ⟨?_, (hp'Vd1.mem_of_mem_vx hx).2⟩
-          obtain hxL | rfl := Walk.endIf_mem_vx hexists hx
-          · push_neg at hxL
-            left
-            exact hxL
-          · right
-            exact hp'finish
-        have := Walk.connected_of_validOn_of_mem hp'Vd Walk.start_vx_mem Walk.finish_vx_mem
-        specialize hVsep p.start ha w.finish hp'finish
-        rw [induce_induce_eq_induce_right _ _ (Set.inter_subset_right.trans ?_), induce_V, ← hp'start] at hVsep
-        exact hVsep this
-        · exact Set.diff_subset
+        refine hsep V hVFin (IsVxSetSeparator.IsPreorder.trans V Ux T ?_ hUxSep)
+        rw [← hUxSep.leftSetV_iff hUx]
+        exact hVsep
       have hFin : G[L ∪ Ux].Finite := by
         refine ⟨?_, ?_⟩
         · apply Set.Finite.union (Set.Finite.subset hfin.vx_fin ?_) hUxFin
@@ -172,60 +246,19 @@ theorem Menger_VxSet {α β : Type*} [DecidableEq α] (G : Graph α β) [hfin : 
           obtain ⟨s, hs, hconn⟩ := hx
           exact Set.diff_subset hconn.mem_left
         · exact Set.Finite.subset hfin.edge_fin (induce_E_le (L ∪ Ux))
-      have htermx : (G.E ∩ {e | ∀ (x : α), G.Inc x e → x = w₁.finish ∨
-        (∃ s ∈ S, G[G.V \ insert w₁.finish U].Connected x s) ∨ x ∈ U}).ncard < G.E.ncard := by
-        sorry
       have := Menger_VxSet (hfin := hFin) (G[L ∪ Ux]) S Ux k hS hUxFin hSUxSepCard
       obtain ⟨Psx, hlenx, hPVdx, hPsxStartSet, hPsxFinishSet⟩ := this
 
-      let Uy := U ∪ {y}
-      have hUy : Uy ⊆ G.V := by
-        simp [Uy, hUV, Set.insert_subset_iff, (Set.diff_subset hxy.vx_mem_right)]
-      let R : Set α := {r | ∃ t ∈ T, G[G.V \ Uy].Connected r t}
+
       have hRV : R ⊆ G.V := by
         rintro r ⟨t, ht, hconn⟩
         exact Set.diff_subset hconn.mem_left
-      have hUyFin : Uy.Finite := hUFin.union (finite_singleton y)
-      have hUyncard : Uy.ncard = k := by sorry
-      -- TODO: U is a separator on G - e. Then, G \ Uy ≤ (G - e) \ U. Connected.le
-      have hUySep : G.IsVxSetSeparator Uy S T := by
-        sorry
-      -- ...
       have hSUySepCard : ∀ (U : Set α), U.Finite → G[R ∪ Uy].IsVxSetSeparator U Uy T → k ≤ U.ncard := by
         rintro V hVFin hVsep
-        refine hsep V hVFin ?_
-        rintro a ha b hb hconn
-        obtain ⟨p, hpVd, rfl, rfl⟩ := Connected.iff_path.mp hconn
-        have hexists : ∃ u ∈ p.val.vx, u ∉ R := by
-          use p.val.start, Walk.start_vx_mem
-          simp only [mem_setOf_eq, not_exists, not_and, R]
-          rintro t ht h
-          exact hUySep p.start ha t ht h
-        sorry
-        -- let w := p.val.endIf (P := fun x ↦ x ∉ R) hexists
-        -- have hp'start : w.start = p.start := endIf_start _
-        -- have hp'finish : w.finish ∈ Uy := by
-        --   obtain ⟨z, hzw, hzL, f, hbtw⟩ := endIf_exists_isBetween_last hexists hpVd sorry -- TODO: w has at least 2 vertices hence nonempty
-        --   have : w.finish ∉ R := endIf_finish hexists
-        --   simp only [mem_setOf_eq, not_exists, not_forall, Decidable.not_not, R] at hzL this
-        --   simp_rw [not_and] at this
-        --   exact foo (hbtw.le (induce_le G Set.diff_subset)) hzL this
-        -- have hp'Vd1 : w.ValidOn (G[G.V \ V]) := endIf_validOn _ hpVd
-        -- have hp'Vd : w.ValidOn (G[(R ∪ Uy) \ V]) := by
-        --   refine ValidOn.induce (hp'Vd1.le (induce_le G Set.diff_subset)) ?_
-        --   rintro x hx
-        --   refine ⟨?_, (hp'Vd1.mem_of_mem_vx hx).2⟩
-        --   obtain hxL | rfl := endIf_mem_vx hexists hx
-        --   · push_neg at hxL
-        --     left
-        --     exact hxL
-        --   · right
-        --     exact hp'finish
-        -- have := Walk.connected_of_validOn_of_mem hp'Vd start_vx_mem finish_vx_mem
-        -- specialize hVsep p.start ha w.finish hp'finish
-        -- rw [induce_induce_eq_induce_right _ _ (Set.inter_subset_right.trans ?_), induce_V, ← hp'start] at hVsep
-        -- exact hVsep this
-        -- · exact Set.diff_subset
+        rw [IsVxSetSeparator.comm] at hVsep hUySep
+        refine hsep V hVFin (IsVxSetSeparator.IsPreorder.trans V Uy S ?_ hUySep).symm
+        rw [← hUySep.leftSetV_iff hUy]
+        exact hVsep
       have hFin : G[R ∪ Uy].Finite := by
         refine ⟨?_, ?_⟩
         · apply Set.Finite.union (Set.Finite.subset hfin.vx_fin ?_) hUyFin
@@ -233,32 +266,55 @@ theorem Menger_VxSet {α β : Type*} [DecidableEq α] (G : Graph α β) [hfin : 
           obtain ⟨s, hs, hconn⟩ := hx
           exact Set.diff_subset hconn.mem_left
         · exact Set.Finite.subset hfin.edge_fin (induce_E_le (R ∪ Uy))
-      have htermy : (G.E ∩ {e | ∀ (x : α), G.Inc x e → x = w₂.start ∨
-        (∃ t ∈ T, G[G.V \ insert w₂.start U].Connected x t) ∨ x ∈ U}).ncard < G.E.ncard := by
-        sorry
-      -- same as above
-      obtain ⟨Psy, hleny, hPVdy, hPsyStartSet, hPsyFinishSet⟩ := Menger_VxSet (hfin := hFin) (G[R ∪ Uy]) Uy T k hUyFin hT hSUySepCard
+      have := Menger_VxSet (hfin := hFin) (G[R ∪ Uy]) Uy T k hUyFin hT hSUySepCard
+      obtain ⟨Psy, hleny, hPVdy, hPsyStartSet, hPsyFinishSet⟩ := this
 
       /- TODO: Now that I have two set of path ensembles, each corresponding to a unique element in
       Ux/Uy, I can append them to get a path ensemble for G. -/
-      have hPsxFinishSet : Psx.FinishSet = Ux := by sorry
-      have hPUStartSet : PU.StartSet = Ux := by sorry
-      have hPUFinishSet : PU.FinishSet = Uy := by sorry
-      have hPsyStartSet : Psy.StartSet = Uy := by sorry
-      have hPsxFin : Psx.Paths.Finite := by sorry
-      have hPUFin : PU.Paths.Finite := by sorry
-      have hPsyFin : Psy.Paths.Finite := by sorry
+      have hPsxFinishSet : Psx.FinishSet = Ux := by
+        apply Set.eq_of_subset_of_ncard_le hPsxFinishSet ?_ hUxFin
+        · rw [hUxncard, PathEnsemble.FinishSet_ncard, hlenx]
+      have hPUStartSet : PU.StartSet = Ux := by
+        simp only [PathEnsemble.insert_startSet, PathEnsemble.nil_startSet, start, union_singleton,
+          PU, Ux]
+        congr
+      have hPUFinishSet : PU.FinishSet = Uy := by
+        simp only [PathEnsemble.insert_finishSet, PathEnsemble.nil_finishSet, finish,
+          union_singleton, PU, Uy]
+        congr
+      have hPsyStartSet : Psy.StartSet = Uy := by
+        apply Set.eq_of_subset_of_ncard_le hPsyStartSet ?_ hUyFin
+        · rw [hUyncard, PathEnsemble.StartSet_ncard, hleny]
+      have hPsxFin : Psx.Paths.Finite := Set.finite_of_ncard_pos (by omega)
+      have hPUFin : PU.Paths.Finite := by
+        apply PathEnsemble.finite_of_finite_graph ?_ hPUVdUxy
+        apply finite_of_finite_induce
+        apply Set.Finite.insert
+        apply Set.Finite.insert _ hUFin
+      have hPsyFin : Psy.Paths.Finite := Set.finite_of_ncard_pos (by omega)
       have hPsxPU : Psx.VxSet ∩ PU.VxSet = Psx.FinishSet := by
-        apply le_antisymm
-        · rintro z ⟨⟨px, hpx, hzpx⟩, pU, hpU, hzpU⟩
+        apply subset_antisymm
+        · rw [hPsxFinishSet]
+          refine (Set.inter_subset_inter (PathEnsemble.VxSet_subset_of_validOn hPVdx) (PathEnsemble.VxSet_subset_of_validOn hPUVdUxy)).trans ?_
+          simp only [induce_V, Uy]
+          suffices (L ∪ Ux) ∩ ({y} ∪ Ux) ⊆ Ux by
+            convert this using 2
+            simp [Ux]
+          rw [← Set.inter_union_distrib_right]
+          simp only [union_subset_iff, subset_refl, and_true]
+          have : L ∩ {y} = ∅ := inter_singleton_eq_empty.mpr hLy
+          rw [this]
+          exact empty_subset Ux
+        · rw [subset_inter_iff]
+          use Psx.finishSet_subset_VxSet
           rw [hPsxFinishSet]
-          have hz1 := Walk.ValidOn.mem_of_mem_vx (hPVdx px hpx) hzpx
-          have hz2 : z ∈ U ∪ {x, y} := by sorry
-          sorry
-        · sorry
+          convert PU.startSet_subset_VxSet
+          exact hPUStartSet.symm
       have hPUPsx : Psx.VxSet ∩ PU.VxSet = PU.StartSet := by
-        sorry
-      have hPUPsy : (Psx.append PU hPsxPU hPUPsx).VxSet ∩ Psy.VxSet = (Psx.append PU hPsxPU hPUPsx).FinishSet := by
+        rwa [hPUStartSet, ← hPsxFinishSet]
+      have hPUPsy : (Psx.append PU hPsxPU hPUPsx).VxSet ∩ Psy.VxSet =
+        (Psx.append PU hPsxPU hPUPsx).FinishSet := by
+
         sorry
       have hPsyPU : (Psx.append PU hPsxPU hPUPsx).VxSet ∩ Psy.VxSet = Psy.StartSet := by
         sorry
@@ -268,14 +324,19 @@ theorem Menger_VxSet {α β : Type*} [DecidableEq α] (G : Graph α β) [hfin : 
       · rw [PathEnsemble.append_ncard_eq_right, ← PathEnsemble.StartSet_ncard, hPsyStartSet]
         exact hUyncard
         exact hPsyFin
-        exact hPsyFin
       · apply PathEnsemble.append_validOn
         · apply PathEnsemble.append_validOn
           · refine hPVdx.le (induce_le G ?_)
             rintro a (ha | ha)
             · exact hLV ha
             · exact hUx ha
-          · sorry
+          · refine (hPUVdUxy.le (induce_le G ?_))
+            rintro a (rfl | rfl | ha)
+            · refine hUx (?_ : x ∈ Ux)
+              simp [Ux]
+            · refine hUy (?_ : y ∈ Uy)
+              simp [Uy]
+            · exact hUV ha
         · refine hPVdy.le (induce_le G ?_)
           rintro a (ha | ha)
           · exact hRV ha
@@ -283,22 +344,51 @@ theorem Menger_VxSet {α β : Type*} [DecidableEq α] (G : Graph α β) [hfin : 
       · rw [PathEnsemble.append_startSet, PathEnsemble.append_startSet]
         exact hPsxStartSet
 
-  · rw [Set.nonempty_iff_ne_empty] at hE
-    have := hsep (G.V ∩ S ∩ T) (by exact Finite.inter_of_right hT (G.V ∩ S)) ?_
-    simp only [ncard_empty, nonpos_iff_eq_zero] at this
-    obtain ⟨U, hU, hUcard⟩ := Set.exists_subset_card_eq this
-    sorry
-    sorry
-    -- use ⟨Path.nil '' U, ?_⟩, ?_, ?_, ?_
-    -- · rintro p ⟨x, hx, rfl⟩
-    --   obtain ⟨⟨hxV, hxS⟩, hxT⟩ := hU hx
-    --   exact ⟨hxS, hxT⟩
-    -- · sorry -- easy
-    -- · simp only
-    --   rwa [Set.ncard_image_of_injective]
-    --   sorry -- have a lemma that nil is injective
-    -- · rintro p ⟨x, hx, rfl⟩
-    --   refine Walk.nil_validOn_iff.mpr ?_
-    --   exact (hU hx).1.1
-    -- · sorry -- easy
-termination_by 1
+  · rw [Set.nonempty_iff_ne_empty, not_not] at hE
+    let X := G.V ∩ S ∩ T
+    have hXfin : X.Finite := Finite.inter_of_right hT (G.V ∩ S)
+    have hXsep : G.IsVxSetSeparator X S T := by
+      rintro a ha b hb hconn
+      rw [connected_iff_eq_mem_of_E_empty] at hconn
+      obtain ⟨rfl, haV, haX⟩ := hconn
+      exact haX ⟨⟨haV, ha⟩, hb⟩
+      · exact subset_eq_empty (induce_le G Set.diff_subset).2.1 hE
+    have hk : k ≤ X.ncard := hsep X hXfin hXsep
+    obtain ⟨Y, hYsu, hYcard⟩ := exists_subset_card_eq hk
+    use PathEnsemble.nil Y β, hYcard ▸ PathEnsemble.nil_ncard, PathEnsemble.nil_validOn ?_, ?_, ?_
+    · exact hYsu.trans <| Set.inter_subset_left.trans Set.inter_subset_left
+    · rw [PathEnsemble.nil_startSet]
+      exact hYsu.trans (Set.inter_subset_left.trans Set.inter_subset_right)
+    · rw [PathEnsemble.nil_finishSet]
+      exact hYsu.trans Set.inter_subset_right
+termination_by G.E.ncard
+decreasing_by
+  · refine lt_of_le_of_lt (Set.ncard_inter_le_ncard_right G.E _ hfin.edge_fin.diff) ?_
+    rw [Set.ncard_diff (by simp only [singleton_subset_iff, he])]
+    simp only [ncard_singleton, tsub_lt_self_iff, lt_one_iff, pos_of_gt, and_true]
+    rw [Set.ncard_pos hfin.edge_fin]
+    exact nonempty_of_mem he
+  · refine ncard_lt_ncard ?_ hfin.edge_fin
+    have hle : G[hUxSep.leftSet ∪ (U ∪ {w₁.finish})] ≤ G := induce_le G <| union_subset hLV hUx
+    refine ssubset_of_subset_not_subset hle.2.1 ?_
+    · rw [not_subset_iff_exists_mem_not_mem]
+      use e, he
+      intro he'
+      have hinc := hxy.inc_right.le (induce_le G diff_subset)
+      rw [← hle.2.2 _ _ he'] at hinc
+      have := hinc.vx_mem
+      unfold L at hLy
+      unfold x at hxney
+      simp [hLy, hyU, hxney.symm] at this
+  · refine ncard_lt_ncard ?_ hfin.edge_fin
+    have hle : G[hUySep.rightSet ∪ (U ∪ {w₂.start})] ≤ G := induce_le G <| union_subset hRV hUy
+    refine ssubset_of_subset_not_subset hle.2.1 ?_
+    · rw [not_subset_iff_exists_mem_not_mem]
+      use e, he
+      intro he'
+      have hinc := hxy.inc_left.le (induce_le G diff_subset)
+      rw [← hle.2.2 _ _ he'] at hinc
+      have := hinc.vx_mem
+      unfold R at hRx
+      unfold y at hxney
+      simp [hRx, hxU, hxney] at this
